Until ecdsa

code/ecdsa/dist/Hacl_P256.c
@@ -2473,172 +2473,6 @@ static void montgomery_multiplication_buffer_by_one_mixed_p256(uint64_t *result)
   cmovznz4_p256(carry, tempBuffer, x_, result);
 }
 
-static void montgomery_multiplication_buffer_by_one_mixed_p384(uint64_t *result)
-{
-  uint32_t len = (uint32_t)6U;
-  KRML_CHECK_SIZE(sizeof (uint64_t), (uint32_t)2U * len);
-  uint64_t t[(uint32_t)2U * len];
-  memset(t, 0U, (uint32_t)2U * len * sizeof (uint64_t));
-  uint64_t *t_low = t;
-  t_low[0U] = (uint64_t)1U;
-  uint32_t len1 = (uint32_t)6U;
-  for (uint32_t i = (uint32_t)1U; i < len1; i++)
-  {
-    t_low[i] = (uint64_t)0U;
-  }
-  uint32_t len10 = (uint32_t)6U;
-  KRML_CHECK_SIZE(sizeof (uint64_t), (uint32_t)2U * len10);
-  uint64_t t2[(uint32_t)2U * len10];
-  memset(t2, 0U, (uint32_t)2U * len10 * sizeof (uint64_t));
-  for (uint32_t i0 = (uint32_t)0U; i0 < len10; i0++)
-  {
-    uint64_t k0 = (uint64_t)4294967297U;
-    uint64_t t10 = t[0U];
-    uint64_t y = (uint64_t)0U;
-    uint64_t temp = (uint64_t)0U;
-    mul_atomic(t10, k0, &y, &temp);
-    uint64_t y_ = y;
-    uint64_t *uu____0 = t2;
-    uint32_t len30 = (uint32_t)6U;
-    for (uint32_t i = (uint32_t)0U; i < len30; i++)
-    {
-      uu____0[i] = (uint64_t)0U;
-    }
-    uint64_t *uu____1 = t2 + (uint32_t)6U;
-    uint32_t len31 = (uint32_t)6U;
-    for (uint32_t i = (uint32_t)0U; i < len31; i++)
-    {
-      uu____1[i] = (uint64_t)0U;
-    }
-    uint64_t
-    p[6U] =
-      {
-        (uint64_t)0xffffffffU, (uint64_t)0xffffffff00000000U, (uint64_t)0xfffffffffffffffeU,
-        (uint64_t)0xffffffffffffffffU, (uint64_t)0xffffffffffffffffU, (uint64_t)0xffffffffffffffffU
-      };
-    uint32_t len32 = (uint32_t)6U;
-    uint64_t bBuffer = y_;
-    uint64_t *partResult = t2;
-    memset(partResult, 0U, (len32 + (uint32_t)1U) * sizeof (uint64_t));
-    for (uint32_t i1 = (uint32_t)0U; i1 < (uint32_t)1U; i1++)
-    {
-      uint64_t bj = (&bBuffer)[i1];
-      uint64_t *res_j = partResult + i1;
-      uint64_t c = (uint64_t)0U;
-      for (uint32_t i = (uint32_t)0U; i < len32 / (uint32_t)4U; i++)
-      {
-        uint64_t a_i = p[(uint32_t)4U * i];
-        uint64_t *res_i0 = res_j + (uint32_t)4U * i;
-        c = mul_wide_add2_u64(a_i, bj, c, res_i0);
-        uint64_t a_i0 = p[(uint32_t)4U * i + (uint32_t)1U];
-        uint64_t *res_i1 = res_j + (uint32_t)4U * i + (uint32_t)1U;
-        c = mul_wide_add2_u64(a_i0, bj, c, res_i1);
-        uint64_t a_i1 = p[(uint32_t)4U * i + (uint32_t)2U];
-        uint64_t *res_i2 = res_j + (uint32_t)4U * i + (uint32_t)2U;
-        c = mul_wide_add2_u64(a_i1, bj, c, res_i2);
-        uint64_t a_i2 = p[(uint32_t)4U * i + (uint32_t)3U];
-        uint64_t *res_i = res_j + (uint32_t)4U * i + (uint32_t)3U;
-        c = mul_wide_add2_u64(a_i2, bj, c, res_i);
-      }
-      for (uint32_t i = len32 / (uint32_t)4U * (uint32_t)4U; i < len32; i++)
-      {
-        uint64_t a_i = p[i];
-        uint64_t *res_i = res_j + i;
-        c = mul_wide_add2_u64(a_i, bj, c, res_i);
-      }
-      uint64_t r = c;
-      partResult[len32 + i1] = r;
-    }
-    uint32_t len33 = (uint32_t)6U * (uint32_t)2U;
-    uint64_t c = (uint64_t)0U;
-    for (uint32_t i = (uint32_t)0U; i < len33 / (uint32_t)4U; i++)
-    {
-      uint64_t t1 = t[(uint32_t)4U * i];
-      uint64_t t210 = t2[(uint32_t)4U * i];
-      uint64_t *res_i0 = t2 + (uint32_t)4U * i;
-      c = Lib_IntTypes_Intrinsics_add_carry_u64(c, t1, t210, res_i0);
-      uint64_t t11 = t[(uint32_t)4U * i + (uint32_t)1U];
-      uint64_t t211 = t2[(uint32_t)4U * i + (uint32_t)1U];
-      uint64_t *res_i1 = t2 + (uint32_t)4U * i + (uint32_t)1U;
-      c = Lib_IntTypes_Intrinsics_add_carry_u64(c, t11, t211, res_i1);
-      uint64_t t12 = t[(uint32_t)4U * i + (uint32_t)2U];
-      uint64_t t212 = t2[(uint32_t)4U * i + (uint32_t)2U];
-      uint64_t *res_i2 = t2 + (uint32_t)4U * i + (uint32_t)2U;
-      c = Lib_IntTypes_Intrinsics_add_carry_u64(c, t12, t212, res_i2);
-      uint64_t t13 = t[(uint32_t)4U * i + (uint32_t)3U];
-      uint64_t t21 = t2[(uint32_t)4U * i + (uint32_t)3U];
-      uint64_t *res_i = t2 + (uint32_t)4U * i + (uint32_t)3U;
-      c = Lib_IntTypes_Intrinsics_add_carry_u64(c, t13, t21, res_i);
-    }
-    for (uint32_t i = len33 / (uint32_t)4U * (uint32_t)4U; i < len33; i++)
-    {
-      uint64_t t1 = t[i];
-      uint64_t t21 = t2[i];
-      uint64_t *res_i = t2 + i;
-      c = Lib_IntTypes_Intrinsics_add_carry_u64(c, t1, t21, res_i);
-    }
-    uint64_t carry = c;
-    uint32_t len3 = (uint32_t)11U;
-    for (uint32_t i = (uint32_t)0U; i < len3; i++)
-    {
-      uint64_t elem = t2[(uint32_t)1U + i];
-      t[i] = elem;
-    }
-    t[len3] = carry;
-  }
-  uint32_t len2 = (uint32_t)6U;
-  uint64_t cin = t[len2];
-  uint64_t *x_ = t;
-  uint32_t len3 = (uint32_t)6U;
-  KRML_CHECK_SIZE(sizeof (uint64_t), len3);
-  uint64_t tempBuffer[len3];
-  memset(tempBuffer, 0U, len3 * sizeof (uint64_t));
-  uint64_t tempBufferForSubborrow = (uint64_t)0U;
-  uint64_t
-  p[6U] =
-    {
-      (uint64_t)0xffffffffU, (uint64_t)0xffffffff00000000U, (uint64_t)0xfffffffffffffffeU,
-      (uint64_t)0xffffffffffffffffU, (uint64_t)0xffffffffffffffffU, (uint64_t)0xffffffffffffffffU
-    };
-  uint32_t len4 = (uint32_t)6U;
-  uint64_t c = (uint64_t)0U;
-  for (uint32_t i = (uint32_t)0U; i < len4 / (uint32_t)4U; i++)
-  {
-    uint64_t t1 = x_[(uint32_t)4U * i];
-    uint64_t t210 = p[(uint32_t)4U * i];
-    uint64_t *res_i0 = tempBuffer + (uint32_t)4U * i;
-    c = Lib_IntTypes_Intrinsics_sub_borrow_u64(c, t1, t210, res_i0);
-    uint64_t t10 = x_[(uint32_t)4U * i + (uint32_t)1U];
-    uint64_t t211 = p[(uint32_t)4U * i + (uint32_t)1U];
-    uint64_t *res_i1 = tempBuffer + (uint32_t)4U * i + (uint32_t)1U;
-    c = Lib_IntTypes_Intrinsics_sub_borrow_u64(c, t10, t211, res_i1);
-    uint64_t t11 = x_[(uint32_t)4U * i + (uint32_t)2U];
-    uint64_t t212 = p[(uint32_t)4U * i + (uint32_t)2U];
-    uint64_t *res_i2 = tempBuffer + (uint32_t)4U * i + (uint32_t)2U;
-    c = Lib_IntTypes_Intrinsics_sub_borrow_u64(c, t11, t212, res_i2);
-    uint64_t t12 = x_[(uint32_t)4U * i + (uint32_t)3U];
-    uint64_t t21 = p[(uint32_t)4U * i + (uint32_t)3U];
-    uint64_t *res_i = tempBuffer + (uint32_t)4U * i + (uint32_t)3U;
-    c = Lib_IntTypes_Intrinsics_sub_borrow_u64(c, t12, t21, res_i);
-  }
-  for (uint32_t i = len4 / (uint32_t)4U * (uint32_t)4U; i < len4; i++)
-  {
-    uint64_t t1 = x_[i];
-    uint64_t t21 = p[i];
-    uint64_t *res_i = tempBuffer + i;
-    c = Lib_IntTypes_Intrinsics_sub_borrow_u64(c, t1, t21, res_i);
-  }
-  uint64_t r = c;
-  uint64_t carry0 = r;
-  uint64_t
-  carry =
-    Lib_IntTypes_Intrinsics_sub_borrow_u64(carry0,
-      cin,
-      (uint64_t)0U,
-      &tempBufferForSubborrow);
-  cmovznz4_p384(carry, tempBuffer, x_, result);
-}
-
 static void
 copy_point_conditional(
   Spec_ECC_Curves_curve c,
@@ -3314,397 +3148,6 @@ point_add_mixed_p256(uint64_t *p, uint64_t *q, uint64_t *result, uint64_t *tempB
   memcpy(result, x3_out, (uint32_t)4U * sizeof (uint64_t));
   memcpy(result + (uint32_t)4U, y3_out, (uint32_t)4U * sizeof (uint64_t));
   memcpy(result + (uint32_t)8U, z3_out, (uint32_t)4U * sizeof (uint64_t));
-}
-
-static inline void
-point_add_mixed_p384(uint64_t *p, uint64_t *q, uint64_t *result, uint64_t *tempBuffer)
-{
-  uint64_t *t12 = tempBuffer;
-  uint64_t *t5 = tempBuffer + (uint32_t)72U;
-  uint64_t *t4 = t12;
-  uint64_t *u10 = t12 + (uint32_t)24U;
-  uint64_t *u20 = t12 + (uint32_t)30U;
-  uint64_t *s10 = t12 + (uint32_t)36U;
-  uint64_t *s20 = t12 + (uint32_t)42U;
-  uint64_t *pX = p;
-  uint64_t *pY = p + (uint32_t)6U;
-  uint64_t *pZ = p + (uint32_t)12U;
-  uint64_t *qX = q;
-  uint64_t *qY = q + (uint32_t)6U;
-  uint64_t *z2Square = t4;
-  uint64_t *z1Square = t4 + (uint32_t)6U;
-  uint64_t *z2Cube = t4 + (uint32_t)12U;
-  uint64_t *z1Cube = t4 + (uint32_t)18U;
-  montgomery_multiplication_buffer_by_one_mixed_p384(z2Square);
-  montgomery_square_buffer_dh_p384(pZ, z1Square);
-  uint32_t len0 = (uint32_t)6U;
-  KRML_CHECK_SIZE(sizeof (uint64_t), (uint32_t)2U * len0);
-  uint64_t t0[(uint32_t)2U * len0];
-  memset(t0, 0U, (uint32_t)2U * len0 * sizeof (uint64_t));
-  uint64_t *t_low0 = t0;
-  memcpy(t_low0, z2Square, len0 * sizeof (uint64_t));
-  uint32_t len1 = (uint32_t)6U;
-  KRML_CHECK_SIZE(sizeof (uint64_t), (uint32_t)2U * len1);
-  uint64_t t20[(uint32_t)2U * len1];
-  memset(t20, 0U, (uint32_t)2U * len1 * sizeof (uint64_t));
-  for (uint32_t i0 = (uint32_t)0U; i0 < len1; i0++)
-  {
-    uint64_t k0 = (uint64_t)4294967297U;
-    uint64_t t10 = t0[0U];
-    uint64_t y = (uint64_t)0U;
-    uint64_t temp = (uint64_t)0U;
-    mul_atomic(t10, k0, &y, &temp);
-    uint64_t y_ = y;
-    uint64_t *uu____0 = t20;
-    uint32_t len30 = (uint32_t)6U;
-    for (uint32_t i = (uint32_t)0U; i < len30; i++)
-    {
-      uu____0[i] = (uint64_t)0U;
-    }
-    uint64_t *uu____1 = t20 + (uint32_t)6U;
-    uint32_t len31 = (uint32_t)6U;
-    for (uint32_t i = (uint32_t)0U; i < len31; i++)
-    {
-      uu____1[i] = (uint64_t)0U;
-    }
-    uint64_t
-    p1[6U] =
-      {
-        (uint64_t)0xffffffffU, (uint64_t)0xffffffff00000000U, (uint64_t)0xfffffffffffffffeU,
-        (uint64_t)0xffffffffffffffffU, (uint64_t)0xffffffffffffffffU, (uint64_t)0xffffffffffffffffU
-      };
-    uint32_t len32 = (uint32_t)6U;
-    uint64_t bBuffer = y_;
-    uint64_t *partResult = t20;
-    memset(partResult, 0U, (len32 + (uint32_t)1U) * sizeof (uint64_t));
-    for (uint32_t i1 = (uint32_t)0U; i1 < (uint32_t)1U; i1++)
-    {
-      uint64_t bj = (&bBuffer)[i1];
-      uint64_t *res_j = partResult + i1;
-      uint64_t c = (uint64_t)0U;
-      for (uint32_t i = (uint32_t)0U; i < len32 / (uint32_t)4U; i++)
-      {
-        uint64_t a_i = p1[(uint32_t)4U * i];
-        uint64_t *res_i0 = res_j + (uint32_t)4U * i;
-        c = mul_wide_add2_u64(a_i, bj, c, res_i0);
-        uint64_t a_i0 = p1[(uint32_t)4U * i + (uint32_t)1U];
-        uint64_t *res_i1 = res_j + (uint32_t)4U * i + (uint32_t)1U;
-        c = mul_wide_add2_u64(a_i0, bj, c, res_i1);
-        uint64_t a_i1 = p1[(uint32_t)4U * i + (uint32_t)2U];
-        uint64_t *res_i2 = res_j + (uint32_t)4U * i + (uint32_t)2U;
-        c = mul_wide_add2_u64(a_i1, bj, c, res_i2);
-        uint64_t a_i2 = p1[(uint32_t)4U * i + (uint32_t)3U];
-        uint64_t *res_i = res_j + (uint32_t)4U * i + (uint32_t)3U;
-        c = mul_wide_add2_u64(a_i2, bj, c, res_i);
-      }
-      for (uint32_t i = len32 / (uint32_t)4U * (uint32_t)4U; i < len32; i++)
-      {
-        uint64_t a_i = p1[i];
-        uint64_t *res_i = res_j + i;
-        c = mul_wide_add2_u64(a_i, bj, c, res_i);
-      }
-      uint64_t r = c;
-      partResult[len32 + i1] = r;
-    }
-    uint32_t len33 = (uint32_t)6U * (uint32_t)2U;
-    uint64_t c = (uint64_t)0U;
-    for (uint32_t i = (uint32_t)0U; i < len33 / (uint32_t)4U; i++)
-    {
-      uint64_t t1 = t0[(uint32_t)4U * i];
-      uint64_t t210 = t20[(uint32_t)4U * i];
-      uint64_t *res_i0 = t20 + (uint32_t)4U * i;
-      c = Lib_IntTypes_Intrinsics_add_carry_u64(c, t1, t210, res_i0);
-      uint64_t t11 = t0[(uint32_t)4U * i + (uint32_t)1U];
-      uint64_t t211 = t20[(uint32_t)4U * i + (uint32_t)1U];
-      uint64_t *res_i1 = t20 + (uint32_t)4U * i + (uint32_t)1U;
-      c = Lib_IntTypes_Intrinsics_add_carry_u64(c, t11, t211, res_i1);
-      uint64_t t13 = t0[(uint32_t)4U * i + (uint32_t)2U];
-      uint64_t t212 = t20[(uint32_t)4U * i + (uint32_t)2U];
-      uint64_t *res_i2 = t20 + (uint32_t)4U * i + (uint32_t)2U;
-      c = Lib_IntTypes_Intrinsics_add_carry_u64(c, t13, t212, res_i2);
-      uint64_t t14 = t0[(uint32_t)4U * i + (uint32_t)3U];
-      uint64_t t21 = t20[(uint32_t)4U * i + (uint32_t)3U];
-      uint64_t *res_i = t20 + (uint32_t)4U * i + (uint32_t)3U;
-      c = Lib_IntTypes_Intrinsics_add_carry_u64(c, t14, t21, res_i);
-    }
-    for (uint32_t i = len33 / (uint32_t)4U * (uint32_t)4U; i < len33; i++)
-    {
-      uint64_t t1 = t0[i];
-      uint64_t t21 = t20[i];
-      uint64_t *res_i = t20 + i;
-      c = Lib_IntTypes_Intrinsics_add_carry_u64(c, t1, t21, res_i);
-    }
-    uint64_t carry = c;
-    uint32_t len3 = (uint32_t)11U;
-    for (uint32_t i = (uint32_t)0U; i < len3; i++)
-    {
-      uint64_t elem = t20[(uint32_t)1U + i];
-      t0[i] = elem;
-    }
-    t0[len3] = carry;
-  }
-  uint32_t len2 = (uint32_t)6U;
-  uint64_t cin = t0[len2];
-  uint64_t *x_0 = t0;
-  uint32_t len30 = (uint32_t)6U;
-  KRML_CHECK_SIZE(sizeof (uint64_t), len30);
-  uint64_t tempBuffer1[len30];
-  memset(tempBuffer1, 0U, len30 * sizeof (uint64_t));
-  uint64_t tempBufferForSubborrow0 = (uint64_t)0U;
-  uint64_t
-  p10[6U] =
-    {
-      (uint64_t)0xffffffffU, (uint64_t)0xffffffff00000000U, (uint64_t)0xfffffffffffffffeU,
-      (uint64_t)0xffffffffffffffffU, (uint64_t)0xffffffffffffffffU, (uint64_t)0xffffffffffffffffU
-    };
-  uint32_t len40 = (uint32_t)6U;
-  uint64_t c0 = (uint64_t)0U;
-  for (uint32_t i = (uint32_t)0U; i < len40 / (uint32_t)4U; i++)
-  {
-    uint64_t t1 = x_0[(uint32_t)4U * i];
-    uint64_t t210 = p10[(uint32_t)4U * i];
-    uint64_t *res_i0 = tempBuffer1 + (uint32_t)4U * i;
-    c0 = Lib_IntTypes_Intrinsics_sub_borrow_u64(c0, t1, t210, res_i0);
-    uint64_t t10 = x_0[(uint32_t)4U * i + (uint32_t)1U];
-    uint64_t t211 = p10[(uint32_t)4U * i + (uint32_t)1U];
-    uint64_t *res_i1 = tempBuffer1 + (uint32_t)4U * i + (uint32_t)1U;
-    c0 = Lib_IntTypes_Intrinsics_sub_borrow_u64(c0, t10, t211, res_i1);
-    uint64_t t11 = x_0[(uint32_t)4U * i + (uint32_t)2U];
-    uint64_t t212 = p10[(uint32_t)4U * i + (uint32_t)2U];
-    uint64_t *res_i2 = tempBuffer1 + (uint32_t)4U * i + (uint32_t)2U;
-    c0 = Lib_IntTypes_Intrinsics_sub_borrow_u64(c0, t11, t212, res_i2);
-    uint64_t t13 = x_0[(uint32_t)4U * i + (uint32_t)3U];
-    uint64_t t21 = p10[(uint32_t)4U * i + (uint32_t)3U];
-    uint64_t *res_i = tempBuffer1 + (uint32_t)4U * i + (uint32_t)3U;
-    c0 = Lib_IntTypes_Intrinsics_sub_borrow_u64(c0, t13, t21, res_i);
-  }
-  for (uint32_t i = len40 / (uint32_t)4U * (uint32_t)4U; i < len40; i++)
-  {
-    uint64_t t1 = x_0[i];
-    uint64_t t21 = p10[i];
-    uint64_t *res_i = tempBuffer1 + i;
-    c0 = Lib_IntTypes_Intrinsics_sub_borrow_u64(c0, t1, t21, res_i);
-  }
-  uint64_t r0 = c0;
-  uint64_t carry0 = r0;
-  uint64_t
-  carry =
-    Lib_IntTypes_Intrinsics_sub_borrow_u64(carry0,
-      cin,
-      (uint64_t)0U,
-      &tempBufferForSubborrow0);
-  cmovznz4_p384(carry, tempBuffer1, x_0, z2Cube);
-  montgomery_multiplication_buffer_dh_p384(z1Square, pZ, z1Cube);
-  montgomery_multiplication_buffer_dh_p384(z2Square, pX, u10);
-  montgomery_multiplication_buffer_dh_p384(z1Square, qX, u20);
-  montgomery_multiplication_buffer_dh_p384(z2Cube, pY, s10);
-  montgomery_multiplication_buffer_dh_p384(z1Cube, qY, s20);
-  uint64_t *temp0 = t12;
-  uint64_t *u1 = t12 + (uint32_t)24U;
-  uint64_t *u2 = t12 + (uint32_t)30U;
-  uint64_t *s11 = t12 + (uint32_t)36U;
-  uint64_t *s2 = t12 + (uint32_t)42U;
-  uint64_t *h = t12 + (uint32_t)48U;
-  uint64_t *r1 = t12 + (uint32_t)54U;
-  uint64_t *uh0 = t12 + (uint32_t)60U;
-  uint64_t *hCube0 = t12 + (uint32_t)66U;
-  felem_sub_p384(u2, u1, h);
-  felem_sub_p384(s2, s11, r1);
-  montgomery_square_buffer_dh_p384(h, temp0);
-  montgomery_multiplication_buffer_dh_p384(temp0, u1, uh0);
-  montgomery_multiplication_buffer_dh_p384(temp0, h, hCube0);
-  uint64_t *h0 = t12 + (uint32_t)48U;
-  uint64_t *r = t12 + (uint32_t)54U;
-  uint64_t *uh = t12 + (uint32_t)60U;
-  uint64_t *hCube = t12 + (uint32_t)66U;
-  uint64_t *s1 = t12 + (uint32_t)36U;
-  uint64_t *x3 = t5;
-  uint64_t *rSquare = t5 + (uint32_t)6U;
-  uint64_t *rH = t5 + (uint32_t)12U;
-  uint64_t *twoUh = t5 + (uint32_t)18U;
-  montgomery_square_buffer_dh_p384(r, rSquare);
-  felem_sub_p384(rSquare, hCube, rH);
-  felem_add_p384(uh, uh, twoUh);
-  felem_sub_p384(rH, twoUh, x3);
-  uint64_t *x30 = t5;
-  uint64_t *y3 = t5 + (uint32_t)6U;
-  uint64_t *s1hCube = t5 + (uint32_t)12U;
-  uint64_t *u1hx3 = t5 + (uint32_t)18U;
-  uint64_t *ru1hx3 = t5 + (uint32_t)24U;
-  montgomery_multiplication_buffer_dh_p384(s1, hCube, s1hCube);
-  felem_sub_p384(uh, x30, u1hx3);
-  montgomery_multiplication_buffer_dh_p384(u1hx3, r, ru1hx3);
-  felem_sub_p384(ru1hx3, s1hCube, y3);
-  uint64_t *z1 = p + (uint32_t)12U;
-  uint64_t *z3 = t5 + (uint32_t)12U;
-  uint64_t *z1z2 = t5 + (uint32_t)18U;
-  uint32_t len = (uint32_t)6U;
-  KRML_CHECK_SIZE(sizeof (uint64_t), (uint32_t)2U * len);
-  uint64_t t[(uint32_t)2U * len];
-  memset(t, 0U, (uint32_t)2U * len * sizeof (uint64_t));
-  uint64_t *t_low = t;
-  memcpy(t_low, z1, len * sizeof (uint64_t));
-  uint32_t len10 = (uint32_t)6U;
-  KRML_CHECK_SIZE(sizeof (uint64_t), (uint32_t)2U * len10);
-  uint64_t t2[(uint32_t)2U * len10];
-  memset(t2, 0U, (uint32_t)2U * len10 * sizeof (uint64_t));
-  for (uint32_t i0 = (uint32_t)0U; i0 < len10; i0++)
-  {
-    uint64_t k0 = (uint64_t)4294967297U;
-    uint64_t t10 = t[0U];
-    uint64_t y = (uint64_t)0U;
-    uint64_t temp = (uint64_t)0U;
-    mul_atomic(t10, k0, &y, &temp);
-    uint64_t y_ = y;
-    uint64_t *uu____2 = t2;
-    uint32_t len31 = (uint32_t)6U;
-    for (uint32_t i = (uint32_t)0U; i < len31; i++)
-    {
-      uu____2[i] = (uint64_t)0U;
-    }
-    uint64_t *uu____3 = t2 + (uint32_t)6U;
-    uint32_t len32 = (uint32_t)6U;
-    for (uint32_t i = (uint32_t)0U; i < len32; i++)
-    {
-      uu____3[i] = (uint64_t)0U;
-    }
-    uint64_t
-    p1[6U] =
-      {
-        (uint64_t)0xffffffffU, (uint64_t)0xffffffff00000000U, (uint64_t)0xfffffffffffffffeU,
-        (uint64_t)0xffffffffffffffffU, (uint64_t)0xffffffffffffffffU, (uint64_t)0xffffffffffffffffU
-      };
-    uint32_t len33 = (uint32_t)6U;
-    uint64_t bBuffer = y_;
-    uint64_t *partResult = t2;
-    memset(partResult, 0U, (len33 + (uint32_t)1U) * sizeof (uint64_t));
-    for (uint32_t i1 = (uint32_t)0U; i1 < (uint32_t)1U; i1++)
-    {
-      uint64_t bj = (&bBuffer)[i1];
-      uint64_t *res_j = partResult + i1;
-      uint64_t c = (uint64_t)0U;
-      for (uint32_t i = (uint32_t)0U; i < len33 / (uint32_t)4U; i++)
-      {
-        uint64_t a_i = p1[(uint32_t)4U * i];
-        uint64_t *res_i0 = res_j + (uint32_t)4U * i;
-        c = mul_wide_add2_u64(a_i, bj, c, res_i0);
-        uint64_t a_i0 = p1[(uint32_t)4U * i + (uint32_t)1U];
-        uint64_t *res_i1 = res_j + (uint32_t)4U * i + (uint32_t)1U;
-        c = mul_wide_add2_u64(a_i0, bj, c, res_i1);
-        uint64_t a_i1 = p1[(uint32_t)4U * i + (uint32_t)2U];
-        uint64_t *res_i2 = res_j + (uint32_t)4U * i + (uint32_t)2U;
-        c = mul_wide_add2_u64(a_i1, bj, c, res_i2);
-        uint64_t a_i2 = p1[(uint32_t)4U * i + (uint32_t)3U];
-        uint64_t *res_i = res_j + (uint32_t)4U * i + (uint32_t)3U;
-        c = mul_wide_add2_u64(a_i2, bj, c, res_i);
-      }
-      for (uint32_t i = len33 / (uint32_t)4U * (uint32_t)4U; i < len33; i++)
-      {
-        uint64_t a_i = p1[i];
-        uint64_t *res_i = res_j + i;
-        c = mul_wide_add2_u64(a_i, bj, c, res_i);
-      }
-      uint64_t r10 = c;
-      partResult[len33 + i1] = r10;
-    }
-    uint32_t len34 = (uint32_t)6U * (uint32_t)2U;
-    uint64_t c = (uint64_t)0U;
-    for (uint32_t i = (uint32_t)0U; i < len34 / (uint32_t)4U; i++)
-    {
-      uint64_t t1 = t[(uint32_t)4U * i];
-      uint64_t t210 = t2[(uint32_t)4U * i];
-      uint64_t *res_i0 = t2 + (uint32_t)4U * i;
-      c = Lib_IntTypes_Intrinsics_add_carry_u64(c, t1, t210, res_i0);
-      uint64_t t11 = t[(uint32_t)4U * i + (uint32_t)1U];
-      uint64_t t211 = t2[(uint32_t)4U * i + (uint32_t)1U];
-      uint64_t *res_i1 = t2 + (uint32_t)4U * i + (uint32_t)1U;
-      c = Lib_IntTypes_Intrinsics_add_carry_u64(c, t11, t211, res_i1);
-      uint64_t t13 = t[(uint32_t)4U * i + (uint32_t)2U];
-      uint64_t t212 = t2[(uint32_t)4U * i + (uint32_t)2U];
-      uint64_t *res_i2 = t2 + (uint32_t)4U * i + (uint32_t)2U;
-      c = Lib_IntTypes_Intrinsics_add_carry_u64(c, t13, t212, res_i2);
-      uint64_t t14 = t[(uint32_t)4U * i + (uint32_t)3U];
-      uint64_t t21 = t2[(uint32_t)4U * i + (uint32_t)3U];
-      uint64_t *res_i = t2 + (uint32_t)4U * i + (uint32_t)3U;
-      c = Lib_IntTypes_Intrinsics_add_carry_u64(c, t14, t21, res_i);
-    }
-    for (uint32_t i = len34 / (uint32_t)4U * (uint32_t)4U; i < len34; i++)
-    {
-      uint64_t t1 = t[i];
-      uint64_t t21 = t2[i];
-      uint64_t *res_i = t2 + i;
-      c = Lib_IntTypes_Intrinsics_add_carry_u64(c, t1, t21, res_i);
-    }
-    uint64_t carry1 = c;
-    uint32_t len3 = (uint32_t)11U;
-    for (uint32_t i = (uint32_t)0U; i < len3; i++)
-    {
-      uint64_t elem = t2[(uint32_t)1U + i];
-      t[i] = elem;
-    }
-    t[len3] = carry1;
-  }
-  uint32_t len20 = (uint32_t)6U;
-  uint64_t cin0 = t[len20];
-  uint64_t *x_ = t;
-  uint32_t len3 = (uint32_t)6U;
-  KRML_CHECK_SIZE(sizeof (uint64_t), len3);
-  uint64_t tempBuffer10[len3];
-  memset(tempBuffer10, 0U, len3 * sizeof (uint64_t));
-  uint64_t tempBufferForSubborrow = (uint64_t)0U;
-  uint64_t
-  p1[6U] =
-    {
-      (uint64_t)0xffffffffU, (uint64_t)0xffffffff00000000U, (uint64_t)0xfffffffffffffffeU,
-      (uint64_t)0xffffffffffffffffU, (uint64_t)0xffffffffffffffffU, (uint64_t)0xffffffffffffffffU
-    };
-  uint32_t len4 = (uint32_t)6U;
-  uint64_t c = (uint64_t)0U;
-  for (uint32_t i = (uint32_t)0U; i < len4 / (uint32_t)4U; i++)
-  {
-    uint64_t t1 = x_[(uint32_t)4U * i];
-    uint64_t t210 = p1[(uint32_t)4U * i];
-    uint64_t *res_i0 = tempBuffer10 + (uint32_t)4U * i;
-    c = Lib_IntTypes_Intrinsics_sub_borrow_u64(c, t1, t210, res_i0);
-    uint64_t t10 = x_[(uint32_t)4U * i + (uint32_t)1U];
-    uint64_t t211 = p1[(uint32_t)4U * i + (uint32_t)1U];
-    uint64_t *res_i1 = tempBuffer10 + (uint32_t)4U * i + (uint32_t)1U;
-    c = Lib_IntTypes_Intrinsics_sub_borrow_u64(c, t10, t211, res_i1);
-    uint64_t t11 = x_[(uint32_t)4U * i + (uint32_t)2U];
-    uint64_t t212 = p1[(uint32_t)4U * i + (uint32_t)2U];
-    uint64_t *res_i2 = tempBuffer10 + (uint32_t)4U * i + (uint32_t)2U;
-    c = Lib_IntTypes_Intrinsics_sub_borrow_u64(c, t11, t212, res_i2);
-    uint64_t t13 = x_[(uint32_t)4U * i + (uint32_t)3U];
-    uint64_t t21 = p1[(uint32_t)4U * i + (uint32_t)3U];
-    uint64_t *res_i = tempBuffer10 + (uint32_t)4U * i + (uint32_t)3U;
-    c = Lib_IntTypes_Intrinsics_sub_borrow_u64(c, t13, t21, res_i);
-  }
-  for (uint32_t i = len4 / (uint32_t)4U * (uint32_t)4U; i < len4; i++)
-  {
-    uint64_t t1 = x_[i];
-    uint64_t t21 = p1[i];
-    uint64_t *res_i = tempBuffer10 + i;
-    c = Lib_IntTypes_Intrinsics_sub_borrow_u64(c, t1, t21, res_i);
-  }
-  uint64_t r10 = c;
-  uint64_t carry00 = r10;
-  uint64_t
-  carry1 =
-    Lib_IntTypes_Intrinsics_sub_borrow_u64(carry00,
-      cin0,
-      (uint64_t)0U,
-      &tempBufferForSubborrow);
-  cmovznz4_p384(carry1, tempBuffer10, x_, z1z2);
-  montgomery_multiplication_buffer_dh_p384(z1z2, h0, z3);
-  uint64_t *x3_out = t5;
-  uint64_t *y3_out = t5 + (uint32_t)6U;
-  uint64_t *z3_out = t5 + (uint32_t)12U;
-  uint64_t *temp = t5 + (uint32_t)18U;
-  copy_point_conditional(Spec_ECC_Curves_P384, x3_out, y3_out, z3_out, q, p, temp);
-  copy_point_conditional1(Spec_ECC_Curves_P384, x3_out, y3_out, z3_out, p, q);
-  memcpy(result, x3_out, (uint32_t)6U * sizeof (uint64_t));
-  memcpy(result + (uint32_t)6U, y3_out, (uint32_t)6U * sizeof (uint64_t));
-  memcpy(result + (uint32_t)12U, z3_out, (uint32_t)6U * sizeof (uint64_t));
 }
 
 static const
@@ -4508,6 +3951,42 @@ montgomery_ladderP256L(uint64_t *p, uint64_t *q, uint8_t *scalar, uint64_t *temp
     point_double_p256(p, p, tempBuffer);
     uint64_t mask0 = (uint64_t)0U - bit;
     uint32_t len = (uint32_t)12U;
+    for (uint32_t i = (uint32_t)0U; i < len; i++)
+    {
+      uint64_t dummy = mask0 & (p[i] ^ q[i]);
+      p[i] = p[i] ^ dummy;
+      q[i] = q[i] ^ dummy;
+    }
+  }
+}
+
+static inline void
+montgomery_ladderP384L(uint64_t *p, uint64_t *q, uint8_t *scalar, uint64_t *tempBuffer)
+{
+  uint32_t cycleLoop = (uint32_t)6U * (uint32_t)8U * (uint32_t)8U;
+  for (uint32_t i0 = (uint32_t)0U; i0 < cycleLoop; i0++)
+  {
+    uint32_t bit0 = (uint32_t)6U * (uint32_t)8U * (uint32_t)8U - (uint32_t)1U - i0;
+    uint64_t
+    bit =
+      (uint64_t)(scalar[(uint32_t)6U
+      * (uint32_t)8U
+      - (uint32_t)1U
+      - bit0 / (uint32_t)8U]
+      >> bit0 % (uint32_t)8U
+      & (uint8_t)1U);
+    uint64_t mask = (uint64_t)0U - bit;
+    uint32_t len0 = (uint32_t)18U;
+    for (uint32_t i = (uint32_t)0U; i < len0; i++)
+    {
+      uint64_t dummy = mask & (p[i] ^ q[i]);
+      p[i] = p[i] ^ dummy;
+      q[i] = q[i] ^ dummy;
+    }
+    point_add_p384(p, q, q, tempBuffer);
+    point_double_p384(p, p, tempBuffer);
+    uint64_t mask0 = (uint64_t)0U - bit;
+    uint32_t len = (uint32_t)18U;
     for (uint32_t i = (uint32_t)0U; i < len; i++)
     {
       uint64_t dummy = mask0 & (p[i] ^ q[i]);
@@ -5823,6 +5302,11 @@ static inline void solinas_reduction_impl_p384(uint64_t *i, uint64_t *o)
   felem_sub_p384(t81, t91, o);
 }
 
+#define ML 0
+#define Radix 1
+
+typedef uint8_t ladder;
+
 static inline void toDomain_p256(uint64_t *value, uint64_t *result)
 {
   uint32_t len = (uint32_t)4U;
@@ -6250,167 +5734,294 @@ static inline void norm_p384(uint64_t *p, uint64_t *resultPoint, uint64_t *tempB
 
 static inline void
 scalarMultiplicationWithoutNorm_p256(
+  ladder l,
   uint64_t *p,
   uint64_t *result,
   void *scalar,
   uint64_t *tempBuffer
 )
 {
-  uint32_t len = (uint32_t)4U;
-  uint64_t *q = tempBuffer;
-  uint64_t *buff = tempBuffer + (uint32_t)3U * len;
-  uint32_t len2 = (uint32_t)4U;
-  uint64_t *p_x = p;
-  uint64_t *p_y = p + len2;
-  uint64_t *p_z = p + (uint32_t)2U * len2;
-  uint64_t *r_x = result;
-  uint64_t *r_y = result + len2;
-  uint64_t *r_z = result + (uint32_t)2U * len2;
-  toDomain_p256(p_x, r_x);
-  toDomain_p256(p_y, r_y);
-  toDomain_p256(p_z, r_z);
-  uint64_t bufferPrecomputed[192U] = { 0U };
-  generatePrecomputedTable(Spec_ECC_Curves_P256, bufferPrecomputed, result, buff);
-  uint32_t
-  bit = (uint32_t)4U * (uint32_t)8U * (uint32_t)8U - (uint32_t)1U - (uint32_t)(uint64_t)0U;
-  uint64_t
-  bit00 =
-    (uint64_t)(((uint8_t *)scalar)[(uint32_t)4U
-    * (uint32_t)8U
-    - (uint32_t)1U
-    - bit / (uint32_t)8U]
-    >> bit % (uint32_t)8U
-    & (uint8_t)1U)
-    << (uint32_t)3U;
-  uint64_t
-  bit10 =
-    (uint64_t)(((uint8_t *)scalar)[(uint32_t)4U
-    * (uint32_t)8U
-    - (uint32_t)1U
-    - (bit - (uint32_t)1U) / (uint32_t)8U]
-    >> (bit - (uint32_t)1U) % (uint32_t)8U
-    & (uint8_t)1U)
-    << (uint32_t)2U;
-  uint64_t
-  bit20 =
-    (uint64_t)(((uint8_t *)scalar)[(uint32_t)4U
-    * (uint32_t)8U
-    - (uint32_t)1U
-    - (bit - (uint32_t)2U) / (uint32_t)8U]
-    >> (bit - (uint32_t)2U) % (uint32_t)8U
-    & (uint8_t)1U)
-    << (uint32_t)1U;
-  uint64_t
-  bit30 =
-    (uint64_t)(((uint8_t *)scalar)[(uint32_t)4U
-    * (uint32_t)8U
-    - (uint32_t)1U
-    - (bit - (uint32_t)3U) / (uint32_t)8U]
-    >> (bit - (uint32_t)3U) % (uint32_t)8U
-    & (uint8_t)1U)
-    << (uint32_t)0U;
-  uint64_t bits = (bit00 ^ bit10) ^ (bit20 ^ bit30);
-  uint64_t *pointToStart = bufferPrecomputed + (uint32_t)(bits * (uint64_t)(uint32_t)12U);
-  memcpy(result, pointToStart, (uint32_t)12U * sizeof (uint64_t));
-  for (uint32_t i0 = (uint32_t)1U; i0 < (uint32_t)64U; i0++)
+  uint32_t len1 = (uint32_t)4U;
+  switch (l)
   {
-    uint32_t
-    bit4 = (uint32_t)4U * (uint32_t)8U * (uint32_t)8U - (uint32_t)1U - (i0 << (uint32_t)2U);
-    uint64_t
-    bit0 =
-      (uint64_t)(((uint8_t *)scalar)[(uint32_t)4U
-      * (uint32_t)8U
-      - (uint32_t)1U
-      - bit4 / (uint32_t)8U]
-      >> bit4 % (uint32_t)8U
-      & (uint8_t)1U)
-      << (uint32_t)3U;
-    uint64_t
-    bit1 =
-      (uint64_t)(((uint8_t *)scalar)[(uint32_t)4U
-      * (uint32_t)8U
-      - (uint32_t)1U
-      - (bit4 - (uint32_t)1U) / (uint32_t)8U]
-      >> (bit4 - (uint32_t)1U) % (uint32_t)8U
-      & (uint8_t)1U)
-      << (uint32_t)2U;
-    uint64_t
-    bit2 =
-      (uint64_t)(((uint8_t *)scalar)[(uint32_t)4U
-      * (uint32_t)8U
-      - (uint32_t)1U
-      - (bit4 - (uint32_t)2U) / (uint32_t)8U]
-      >> (bit4 - (uint32_t)2U) % (uint32_t)8U
-      & (uint8_t)1U)
-      << (uint32_t)1U;
-    uint64_t
-    bit3 =
-      (uint64_t)(((uint8_t *)scalar)[(uint32_t)4U
-      * (uint32_t)8U
-      - (uint32_t)1U
-      - (bit4 - (uint32_t)3U) / (uint32_t)8U]
-      >> (bit4 - (uint32_t)3U) % (uint32_t)8U
-      & (uint8_t)1U)
-      << (uint32_t)0U;
-    uint64_t bits1 = (bit0 ^ bit1) ^ (bit2 ^ bit3);
-    uint64_t pointToAdd[12U] = { 0U };
-    for (uint32_t i = (uint32_t)0U; i < (uint32_t)16U; i++)
-    {
-      uint64_t mask = FStar_UInt64_eq_mask(bits1, (uint64_t)i);
-      uint64_t *lut_cmb_x = bufferPrecomputed + i * (uint32_t)(krml_checked_int_t)12;
-      uint64_t *lut_cmb_y = bufferPrecomputed + i * (uint32_t)(krml_checked_int_t)12 + (uint32_t)4U;
-      uint64_t *lut_cmb_z = bufferPrecomputed + i * (uint32_t)(krml_checked_int_t)12 + (uint32_t)8U;
-      copy_conditional_p256_l(pointToAdd, lut_cmb_x, mask);
-      copy_conditional_p256_l(pointToAdd + (uint32_t)4U, lut_cmb_y, mask);
-      copy_conditional_p256_l(pointToAdd + (uint32_t)8U, lut_cmb_z, mask);
-    }
-    point_double_p256(result, result, buff);
-    point_double_p256(result, result, buff);
-    point_double_p256(result, result, buff);
-    point_double_p256(result, result, buff);
-    point_add_p256(pointToAdd, result, result, buff);
+    case ML:
+      {
+        uint64_t *q = tempBuffer;
+        uint64_t *buff = tempBuffer + (uint32_t)3U * len1;
+        uint32_t len2 = (uint32_t)4U;
+        uint64_t *x = q;
+        uint64_t *y = q + len2;
+        uint64_t *z = q + (uint32_t)2U * len2;
+        uint32_t len3 = (uint32_t)4U;
+        for (uint32_t i = (uint32_t)0U; i < len3; i++)
+        {
+          x[i] = (uint64_t)0U;
+        }
+        uint32_t len30 = (uint32_t)4U;
+        for (uint32_t i = (uint32_t)0U; i < len30; i++)
+        {
+          y[i] = (uint64_t)0U;
+        }
+        uint32_t len31 = (uint32_t)4U;
+        for (uint32_t i = (uint32_t)0U; i < len31; i++)
+        {
+          z[i] = (uint64_t)0U;
+        }
+        uint32_t len20 = (uint32_t)4U;
+        uint64_t *p_x = p;
+        uint64_t *p_y = p + len20;
+        uint64_t *p_z = p + (uint32_t)2U * len20;
+        uint64_t *r_x = result;
+        uint64_t *r_y = result + len20;
+        uint64_t *r_z = result + (uint32_t)2U * len20;
+        toDomain_p256(p_x, r_x);
+        toDomain_p256(p_y, r_y);
+        toDomain_p256(p_z, r_z);
+        montgomery_ladderP256L(q, result, (uint8_t *)scalar, buff);
+        memcpy(result, q, (uint32_t)12U * sizeof (uint64_t));
+        break;
+      }
+    case Radix:
+      {
+        uint32_t len2 = (uint32_t)4U;
+        uint64_t *p_x = p;
+        uint64_t *p_y = p + len2;
+        uint64_t *p_z = p + (uint32_t)2U * len2;
+        uint64_t *r_x = result;
+        uint64_t *r_y = result + len2;
+        uint64_t *r_z = result + (uint32_t)2U * len2;
+        toDomain_p256(p_x, r_x);
+        toDomain_p256(p_y, r_y);
+        toDomain_p256(p_z, r_z);
+        uint64_t bufferPrecomputed[192U] = { 0U };
+        generatePrecomputedTable(Spec_ECC_Curves_P256, bufferPrecomputed, result, tempBuffer);
+        uint32_t
+        bit = (uint32_t)4U * (uint32_t)8U * (uint32_t)8U - (uint32_t)1U - (uint32_t)(uint64_t)0U;
+        uint64_t
+        bit00 =
+          (uint64_t)(((uint8_t *)scalar)[(uint32_t)4U
+          * (uint32_t)8U
+          - (uint32_t)1U
+          - bit / (uint32_t)8U]
+          >> bit % (uint32_t)8U
+          & (uint8_t)1U)
+          << (uint32_t)3U;
+        uint64_t
+        bit10 =
+          (uint64_t)(((uint8_t *)scalar)[(uint32_t)4U
+          * (uint32_t)8U
+          - (uint32_t)1U
+          - (bit - (uint32_t)1U) / (uint32_t)8U]
+          >> (bit - (uint32_t)1U) % (uint32_t)8U
+          & (uint8_t)1U)
+          << (uint32_t)2U;
+        uint64_t
+        bit20 =
+          (uint64_t)(((uint8_t *)scalar)[(uint32_t)4U
+          * (uint32_t)8U
+          - (uint32_t)1U
+          - (bit - (uint32_t)2U) / (uint32_t)8U]
+          >> (bit - (uint32_t)2U) % (uint32_t)8U
+          & (uint8_t)1U)
+          << (uint32_t)1U;
+        uint64_t
+        bit30 =
+          (uint64_t)(((uint8_t *)scalar)[(uint32_t)4U
+          * (uint32_t)8U
+          - (uint32_t)1U
+          - (bit - (uint32_t)3U) / (uint32_t)8U]
+          >> (bit - (uint32_t)3U) % (uint32_t)8U
+          & (uint8_t)1U)
+          << (uint32_t)0U;
+        uint64_t bits = (bit00 ^ bit10) ^ (bit20 ^ bit30);
+        uint64_t *pointToStart = bufferPrecomputed + (uint32_t)(bits * (uint64_t)(uint32_t)12U);
+        memcpy(result, pointToStart, (uint32_t)12U * sizeof (uint64_t));
+        for (uint32_t i0 = (uint32_t)1U; i0 < (uint32_t)64U; i0++)
+        {
+          uint32_t
+          bit4 = (uint32_t)4U * (uint32_t)8U * (uint32_t)8U - (uint32_t)1U - (i0 << (uint32_t)2U);
+          uint64_t
+          bit0 =
+            (uint64_t)(((uint8_t *)scalar)[(uint32_t)4U
+            * (uint32_t)8U
+            - (uint32_t)1U
+            - bit4 / (uint32_t)8U]
+            >> bit4 % (uint32_t)8U
+            & (uint8_t)1U)
+            << (uint32_t)3U;
+          uint64_t
+          bit1 =
+            (uint64_t)(((uint8_t *)scalar)[(uint32_t)4U
+            * (uint32_t)8U
+            - (uint32_t)1U
+            - (bit4 - (uint32_t)1U) / (uint32_t)8U]
+            >> (bit4 - (uint32_t)1U) % (uint32_t)8U
+            & (uint8_t)1U)
+            << (uint32_t)2U;
+          uint64_t
+          bit2 =
+            (uint64_t)(((uint8_t *)scalar)[(uint32_t)4U
+            * (uint32_t)8U
+            - (uint32_t)1U
+            - (bit4 - (uint32_t)2U) / (uint32_t)8U]
+            >> (bit4 - (uint32_t)2U) % (uint32_t)8U
+            & (uint8_t)1U)
+            << (uint32_t)1U;
+          uint64_t
+          bit3 =
+            (uint64_t)(((uint8_t *)scalar)[(uint32_t)4U
+            * (uint32_t)8U
+            - (uint32_t)1U
+            - (bit4 - (uint32_t)3U) / (uint32_t)8U]
+            >> (bit4 - (uint32_t)3U) % (uint32_t)8U
+            & (uint8_t)1U)
+            << (uint32_t)0U;
+          uint64_t bits1 = (bit0 ^ bit1) ^ (bit2 ^ bit3);
+          uint64_t pointToAdd[12U] = { 0U };
+          for (uint32_t i = (uint32_t)0U; i < (uint32_t)16U; i++)
+          {
+            uint64_t mask = FStar_UInt64_eq_mask(bits1, (uint64_t)i);
+            uint64_t *lut_cmb_x = bufferPrecomputed + i * (uint32_t)(krml_checked_int_t)12;
+            uint64_t
+            *lut_cmb_y = bufferPrecomputed + i * (uint32_t)(krml_checked_int_t)12 + (uint32_t)4U;
+            uint64_t
+            *lut_cmb_z = bufferPrecomputed + i * (uint32_t)(krml_checked_int_t)12 + (uint32_t)8U;
+            copy_conditional_p256_l(pointToAdd, lut_cmb_x, mask);
+            copy_conditional_p256_l(pointToAdd + (uint32_t)4U, lut_cmb_y, mask);
+            copy_conditional_p256_l(pointToAdd + (uint32_t)8U, lut_cmb_z, mask);
+          }
+          point_double_p256(result, result, tempBuffer);
+          point_double_p256(result, result, tempBuffer);
+          point_double_p256(result, result, tempBuffer);
+          point_double_p256(result, result, tempBuffer);
+          point_add_p256(pointToAdd, result, result, tempBuffer);
+        }
+        break;
+      }
+    default:
+      {
+        KRML_HOST_EPRINTF("KreMLin incomplete match at %s:%d\n", __FILE__, __LINE__);
+        KRML_HOST_EXIT(253U);
+      }
   }
-  memcpy(result, q, (uint32_t)12U * sizeof (uint64_t));
 }
 
 static inline void
-secretToPublicWithoutNorm_p256(uint64_t *result, void *scalar, uint64_t *tempBuffer)
+secretToPublicWithoutNorm_p256(ladder l, uint64_t *result, void *scalar, uint64_t *tempBuffer)
 {
   uint32_t len = (uint32_t)4U;
   uint64_t *q = tempBuffer;
   uint64_t *buff = tempBuffer + (uint32_t)3U * len;
-  uint32_t len1 = (uint32_t)4U;
-  uint64_t *x = result;
-  uint64_t *y = result + len1;
-  uint64_t *z = result + (uint32_t)2U * len1;
-  uint32_t len2 = (uint32_t)4U;
-  for (uint32_t i = (uint32_t)0U; i < len2; i++)
+  switch (l)
   {
-    x[i] = (uint64_t)0U;
+    case ML:
+      {
+        uint32_t len1 = (uint32_t)4U;
+        uint64_t *x = q;
+        uint64_t *y = q + len1;
+        uint64_t *z = q + (uint32_t)2U * len1;
+        uint32_t len2 = (uint32_t)4U;
+        for (uint32_t i = (uint32_t)0U; i < len2; i++)
+        {
+          x[i] = (uint64_t)0U;
+        }
+        uint32_t len20 = (uint32_t)4U;
+        for (uint32_t i = (uint32_t)0U; i < len20; i++)
+        {
+          y[i] = (uint64_t)0U;
+        }
+        uint32_t len21 = (uint32_t)4U;
+        for (uint32_t i = (uint32_t)0U; i < len21; i++)
+        {
+          z[i] = (uint64_t)0U;
+        }
+        result[0U] = (uint64_t)0x79e730d418a9143cU;
+        result[1U] = (uint64_t)0x75ba95fc5fedb601U;
+        result[2U] = (uint64_t)0x79fb732b77622510U;
+        result[3U] = (uint64_t)0x18905f76a53755c6U;
+        result[4U] = (uint64_t)0xddf25357ce95560aU;
+        result[5U] = (uint64_t)0x8b4ab8e4ba19e45cU;
+        result[6U] = (uint64_t)0xd2e88688dd21f325U;
+        result[7U] = (uint64_t)0x8571ff1825885d85U;
+        result[8U] = (uint64_t)0x1U;
+        result[9U] = (uint64_t)0xffffffff00000000U;
+        result[10U] = (uint64_t)0xffffffffffffffffU;
+        result[11U] = (uint64_t)0xfffffffeU;
+        montgomery_ladderP256L(q, result, (uint8_t *)scalar, buff);
+        memcpy(result, q, (uint32_t)12U * sizeof (uint64_t));
+        break;
+      }
+    case Radix:
+      {
+        uint32_t
+        bit =
+          (uint32_t)4U
+          * (uint32_t)8U
+          * (uint32_t)8U
+          - (uint32_t)1U
+          - ((uint32_t)(krml_checked_int_t)0 << (uint32_t)2U);
+        uint64_t
+        bit0 =
+          (uint64_t)(((uint8_t *)scalar)[(uint32_t)4U
+          * (uint32_t)8U
+          - (uint32_t)1U
+          - bit / (uint32_t)8U]
+          >> bit % (uint32_t)8U
+          & (uint8_t)1U)
+          << (uint32_t)3U;
+        uint64_t
+        bit1 =
+          (uint64_t)(((uint8_t *)scalar)[(uint32_t)4U
+          * (uint32_t)8U
+          - (uint32_t)1U
+          - (bit - (uint32_t)1U) / (uint32_t)8U]
+          >> (bit - (uint32_t)1U) % (uint32_t)8U
+          & (uint8_t)1U)
+          << (uint32_t)2U;
+        uint64_t
+        bit2 =
+          (uint64_t)(((uint8_t *)scalar)[(uint32_t)4U
+          * (uint32_t)8U
+          - (uint32_t)1U
+          - (bit - (uint32_t)2U) / (uint32_t)8U]
+          >> (bit - (uint32_t)2U) % (uint32_t)8U
+          & (uint8_t)1U)
+          << (uint32_t)1U;
+        uint64_t
+        bit3 =
+          (uint64_t)(((uint8_t *)scalar)[(uint32_t)4U
+          * (uint32_t)8U
+          - (uint32_t)1U
+          - (bit - (uint32_t)3U) / (uint32_t)8U]
+          >> (bit - (uint32_t)3U) % (uint32_t)8U
+          & (uint8_t)1U)
+          << (uint32_t)0U;
+        uint64_t bits = (bit0 ^ bit1) ^ (bit2 ^ bit3);
+        const uint64_t *pointToStart = points_radix_16 + (uint32_t)(bits * (uint64_t)(uint32_t)8U);
+        memcpy(result, (uint64_t *)pointToStart, (uint32_t)8U * sizeof (uint64_t));
+        result[8U] = (uint64_t)1U;
+        result[9U] = (uint64_t)0U;
+        result[10U] = (uint64_t)0U;
+        result[11U] = (uint64_t)0U;
+        for (uint32_t i = (uint32_t)1U; i < (uint32_t)64U; i++)
+        {
+          uint64_t pointToAdd[8U] = { 0U };
+          getPointPrecomputedMixed_p256(scalar, i, pointToAdd);
+          point_double_p256(result, result, buff);
+          point_double_p256(result, result, buff);
+          point_double_p256(result, result, buff);
+          point_double_p256(result, result, buff);
+          point_add_mixed_p256(result, pointToAdd, result, buff);
+        }
+        memcpy(q, result, (uint32_t)12U * sizeof (uint64_t));
+        break;
+      }
+    default:
+      {
+        KRML_HOST_EPRINTF("KreMLin incomplete match at %s:%d\n", __FILE__, __LINE__);
+        KRML_HOST_EXIT(253U);
+      }
   }
-  uint32_t len20 = (uint32_t)4U;
-  for (uint32_t i = (uint32_t)0U; i < len20; i++)
-  {
-    y[i] = (uint64_t)0U;
-  }
-  uint32_t len21 = (uint32_t)4U;
-  for (uint32_t i = (uint32_t)0U; i < len21; i++)
-  {
-    z[i] = (uint64_t)0U;
-  }
-  q[0U] = (uint64_t)0x79e730d418a9143cU;
-  q[1U] = (uint64_t)0x75ba95fc5fedb601U;
-  q[2U] = (uint64_t)0x79fb732b77622510U;
-  q[3U] = (uint64_t)0x18905f76a53755c6U;
-  q[4U] = (uint64_t)0xddf25357ce95560aU;
-  q[5U] = (uint64_t)0x8b4ab8e4ba19e45cU;
-  q[6U] = (uint64_t)0xd2e88688dd21f325U;
-  q[7U] = (uint64_t)0x8571ff1825885d85U;
-  q[8U] = (uint64_t)0x1U;
-  q[9U] = (uint64_t)0xffffffff00000000U;
-  q[10U] = (uint64_t)0xffffffffffffffffU;
-  q[11U] = (uint64_t)0xfffffffeU;
-  montgomery_ladderP256L(result, q, (uint8_t *)scalar, buff);
 }
 
 static inline void fromFormPoint_p256(uint64_t *i, uint8_t *o)
@@ -6890,7 +6501,7 @@ Hacl_P256_ecdsa_sign_p256_sha2(
   uint64_t result1[(uint32_t)3U * len21];
   memset(result1, 0U, (uint32_t)3U * len21 * sizeof (uint64_t));
   uint64_t *tempForNorm = tempBuffer;
-  secretToPublicWithoutNorm_p256(result1, (void *)k, tempBuffer);
+  secretToPublicWithoutNorm_p256(ML, result1, (void *)k, tempBuffer);
   uint64_t *xf = result1;
   uint64_t *zf = result1 + (uint32_t)8U;
   uint64_t *z2f = tempForNorm + (uint32_t)4U;
@@ -7037,7 +6648,7 @@ Hacl_P256_ecdsa_sign_p256_sha384(
   uint64_t result1[(uint32_t)3U * len21];
   memset(result1, 0U, (uint32_t)3U * len21 * sizeof (uint64_t));
   uint64_t *tempForNorm = tempBuffer;
-  secretToPublicWithoutNorm_p256(result1, (void *)k, tempBuffer);
+  secretToPublicWithoutNorm_p256(ML, result1, (void *)k, tempBuffer);
   uint64_t *xf = result1;
   uint64_t *zf = result1 + (uint32_t)8U;
   uint64_t *z2f = tempForNorm + (uint32_t)4U;
@@ -7184,7 +6795,7 @@ Hacl_P256_ecdsa_sign_p256_sha512(
   uint64_t result1[(uint32_t)3U * len21];
   memset(result1, 0U, (uint32_t)3U * len21 * sizeof (uint64_t));
   uint64_t *tempForNorm = tempBuffer;
-  secretToPublicWithoutNorm_p256(result1, (void *)k, tempBuffer);
+  secretToPublicWithoutNorm_p256(ML, result1, (void *)k, tempBuffer);
   uint64_t *xf = result1;
   uint64_t *zf = result1 + (uint32_t)8U;
   uint64_t *z2f = tempForNorm + (uint32_t)4U;
@@ -7333,7 +6944,7 @@ Hacl_P256_ecdsa_sign_p256_without_hash(
   uint64_t result1[(uint32_t)3U * len21];
   memset(result1, 0U, (uint32_t)3U * len21 * sizeof (uint64_t));
   uint64_t *tempForNorm = tempBuffer;
-  secretToPublicWithoutNorm_p256(result1, (void *)k, tempBuffer);
+  secretToPublicWithoutNorm_p256(ML, result1, (void *)k, tempBuffer);
   uint64_t *xf = result1;
   uint64_t *zf = result1 + (uint32_t)8U;
   uint64_t *z2f = tempForNorm + (uint32_t)4U;
@@ -7737,8 +7348,8 @@ Hacl_P256_ecdsa_verif_p256_sha2(
       memset(points, 0U, len4 * (uint32_t)6U * sizeof (uint64_t));
       uint64_t *pointU1G = points;
       uint64_t *pointU2Q = points + (uint32_t)12U;
-      secretToPublicWithoutNorm_p256(pointU1G, (void *)u1, tempBuffer1);
-      scalarMultiplicationWithoutNorm_p256(publicKeyBuffer, pointU2Q, (void *)u2, tempBuffer1);
+      secretToPublicWithoutNorm_p256(ML, pointU1G, (void *)u1, tempBuffer1);
+      scalarMultiplicationWithoutNorm_p256(ML, publicKeyBuffer, pointU2Q, (void *)u2, tempBuffer1);
       uint64_t *tempBuffer17 = tempBuffer1;
       uint64_t *p = points;
       uint64_t *q = points + (uint32_t)12U;
@@ -9470,8 +9081,8 @@ Hacl_P256_ecdsa_verif_p256_sha384(
       memset(points, 0U, len4 * (uint32_t)6U * sizeof (uint64_t));
       uint64_t *pointU1G = points;
       uint64_t *pointU2Q = points + (uint32_t)12U;
-      secretToPublicWithoutNorm_p256(pointU1G, (void *)u1, tempBuffer1);
-      scalarMultiplicationWithoutNorm_p256(publicKeyBuffer, pointU2Q, (void *)u2, tempBuffer1);
+      secretToPublicWithoutNorm_p256(ML, pointU1G, (void *)u1, tempBuffer1);
+      scalarMultiplicationWithoutNorm_p256(ML, publicKeyBuffer, pointU2Q, (void *)u2, tempBuffer1);
       uint64_t *tempBuffer17 = tempBuffer1;
       uint64_t *p = points;
       uint64_t *q = points + (uint32_t)12U;
@@ -11203,8 +10814,8 @@ Hacl_P256_ecdsa_verif_p256_sha512(
       memset(points, 0U, len4 * (uint32_t)6U * sizeof (uint64_t));
       uint64_t *pointU1G = points;
       uint64_t *pointU2Q = points + (uint32_t)12U;
-      secretToPublicWithoutNorm_p256(pointU1G, (void *)u1, tempBuffer1);
-      scalarMultiplicationWithoutNorm_p256(publicKeyBuffer, pointU2Q, (void *)u2, tempBuffer1);
+      secretToPublicWithoutNorm_p256(ML, pointU1G, (void *)u1, tempBuffer1);
+      scalarMultiplicationWithoutNorm_p256(ML, publicKeyBuffer, pointU2Q, (void *)u2, tempBuffer1);
       uint64_t *tempBuffer17 = tempBuffer1;
       uint64_t *p = points;
       uint64_t *q = points + (uint32_t)12U;
@@ -12938,8 +12549,8 @@ Hacl_P256_ecdsa_verif_without_hash(
       memset(points, 0U, len4 * (uint32_t)6U * sizeof (uint64_t));
       uint64_t *pointU1G = points;
       uint64_t *pointU2Q = points + (uint32_t)12U;
-      secretToPublicWithoutNorm_p256(pointU1G, (void *)u1, tempBuffer1);
-      scalarMultiplicationWithoutNorm_p256(publicKeyBuffer, pointU2Q, (void *)u2, tempBuffer1);
+      secretToPublicWithoutNorm_p256(ML, pointU1G, (void *)u1, tempBuffer1);
+      scalarMultiplicationWithoutNorm_p256(ML, publicKeyBuffer, pointU2Q, (void *)u2, tempBuffer1);
       uint64_t *tempBuffer17 = tempBuffer1;
       uint64_t *p = points;
       uint64_t *q = points + (uint32_t)12U;
@@ -14406,67 +14017,38 @@ uint64_t Hacl_P256_ecp256dh_i_ml(uint8_t *result, uint8_t *scalar)
   uint32_t len1 = (uint32_t)4U;
   uint64_t *q = tempBuffer;
   uint64_t *buff = tempBuffer + (uint32_t)3U * len1;
-  uint32_t
-  bit =
-    (uint32_t)4U
-    * (uint32_t)8U
-    * (uint32_t)8U
-    - (uint32_t)1U
-    - ((uint32_t)(krml_checked_int_t)0 << (uint32_t)2U);
-  uint64_t
-  bit0 =
-    (uint64_t)(scalar[(uint32_t)4U
-    * (uint32_t)8U
-    - (uint32_t)1U
-    - bit / (uint32_t)8U]
-    >> bit % (uint32_t)8U
-    & (uint8_t)1U)
-    << (uint32_t)3U;
-  uint64_t
-  bit1 =
-    (uint64_t)(scalar[(uint32_t)4U
-    * (uint32_t)8U
-    - (uint32_t)1U
-    - (bit - (uint32_t)1U) / (uint32_t)8U]
-    >> (bit - (uint32_t)1U) % (uint32_t)8U
-    & (uint8_t)1U)
-    << (uint32_t)2U;
-  uint64_t
-  bit2 =
-    (uint64_t)(scalar[(uint32_t)4U
-    * (uint32_t)8U
-    - (uint32_t)1U
-    - (bit - (uint32_t)2U) / (uint32_t)8U]
-    >> (bit - (uint32_t)2U) % (uint32_t)8U
-    & (uint8_t)1U)
-    << (uint32_t)1U;
-  uint64_t
-  bit3 =
-    (uint64_t)(scalar[(uint32_t)4U
-    * (uint32_t)8U
-    - (uint32_t)1U
-    - (bit - (uint32_t)3U) / (uint32_t)8U]
-    >> (bit - (uint32_t)3U) % (uint32_t)8U
-    & (uint8_t)1U)
-    << (uint32_t)0U;
-  uint64_t bits = (bit0 ^ bit1) ^ (bit2 ^ bit3);
-  const uint64_t *pointToStart = points_radix_16 + (uint32_t)(bits * (uint64_t)(uint32_t)8U);
-  memcpy(resultBuffer, (uint64_t *)pointToStart, (uint32_t)8U * sizeof (uint64_t));
-  resultBuffer[8U] = (uint64_t)1U;
-  resultBuffer[9U] = (uint64_t)0U;
-  resultBuffer[10U] = (uint64_t)0U;
-  resultBuffer[11U] = (uint64_t)0U;
-  for (uint32_t i = (uint32_t)1U; i < (uint32_t)64U; i++)
+  uint32_t len20 = (uint32_t)4U;
+  uint64_t *x = q;
+  uint64_t *y = q + len20;
+  uint64_t *z = q + (uint32_t)2U * len20;
+  uint32_t len3 = (uint32_t)4U;
+  for (uint32_t i = (uint32_t)0U; i < len3; i++)
   {
-    uint64_t pointToAdd[8U] = { 0U };
-    getPointPrecomputedMixed_p256((void *)scalar, i, pointToAdd);
-    point_double_p256(resultBuffer, resultBuffer, buff);
-    point_double_p256(resultBuffer, resultBuffer, buff);
-    point_double_p256(resultBuffer, resultBuffer, buff);
-    point_double_p256(resultBuffer, resultBuffer, buff);
-    point_add_mixed_p256(resultBuffer, pointToAdd, resultBuffer, buff);
+    x[i] = (uint64_t)0U;
   }
-  memcpy(q, resultBuffer, (uint32_t)12U * sizeof (uint64_t));
+  uint32_t len30 = (uint32_t)4U;
+  for (uint32_t i = (uint32_t)0U; i < len30; i++)
+  {
+    y[i] = (uint64_t)0U;
+  }
+  uint32_t len31 = (uint32_t)4U;
+  for (uint32_t i = (uint32_t)0U; i < len31; i++)
+  {
+    z[i] = (uint64_t)0U;
+  }
+  resultBuffer[0U] = (uint64_t)0x79e730d418a9143cU;
+  resultBuffer[1U] = (uint64_t)0x75ba95fc5fedb601U;
+  resultBuffer[2U] = (uint64_t)0x79fb732b77622510U;
+  resultBuffer[3U] = (uint64_t)0x18905f76a53755c6U;
+  resultBuffer[4U] = (uint64_t)0xddf25357ce95560aU;
+  resultBuffer[5U] = (uint64_t)0x8b4ab8e4ba19e45cU;
+  resultBuffer[6U] = (uint64_t)0xd2e88688dd21f325U;
+  resultBuffer[7U] = (uint64_t)0x8571ff1825885d85U;
+  resultBuffer[8U] = (uint64_t)0x1U;
+  resultBuffer[9U] = (uint64_t)0xffffffff00000000U;
+  resultBuffer[10U] = (uint64_t)0xffffffffffffffffU;
+  resultBuffer[11U] = (uint64_t)0xfffffffeU;
+  montgomery_ladderP256L(q, resultBuffer, scalar, buff);
   norm_p256(q, resultBuffer, buff);
   uint32_t len10 = (uint32_t)4U;
   uint32_t start = len10 * (uint32_t)2U;
@@ -14599,67 +14181,44 @@ uint64_t Hacl_P256_ecp384dh_i(uint8_t *result, uint8_t *scalar)
   uint32_t len1 = (uint32_t)6U;
   uint64_t *q = tempBuffer;
   uint64_t *buff = tempBuffer + (uint32_t)3U * len1;
-  uint32_t
-  bit =
-    (uint32_t)6U
-    * (uint32_t)8U
-    * (uint32_t)8U
-    - (uint32_t)1U
-    - ((uint32_t)(krml_checked_int_t)0 << (uint32_t)2U);
-  uint64_t
-  bit0 =
-    (uint64_t)(scalar[(uint32_t)6U
-    * (uint32_t)8U
-    - (uint32_t)1U
-    - bit / (uint32_t)8U]
-    >> bit % (uint32_t)8U
-    & (uint8_t)1U)
-    << (uint32_t)3U;
-  uint64_t
-  bit1 =
-    (uint64_t)(scalar[(uint32_t)6U
-    * (uint32_t)8U
-    - (uint32_t)1U
-    - (bit - (uint32_t)1U) / (uint32_t)8U]
-    >> (bit - (uint32_t)1U) % (uint32_t)8U
-    & (uint8_t)1U)
-    << (uint32_t)2U;
-  uint64_t
-  bit2 =
-    (uint64_t)(scalar[(uint32_t)6U
-    * (uint32_t)8U
-    - (uint32_t)1U
-    - (bit - (uint32_t)2U) / (uint32_t)8U]
-    >> (bit - (uint32_t)2U) % (uint32_t)8U
-    & (uint8_t)1U)
-    << (uint32_t)1U;
-  uint64_t
-  bit3 =
-    (uint64_t)(scalar[(uint32_t)6U
-    * (uint32_t)8U
-    - (uint32_t)1U
-    - (bit - (uint32_t)3U) / (uint32_t)8U]
-    >> (bit - (uint32_t)3U) % (uint32_t)8U
-    & (uint8_t)1U)
-    << (uint32_t)0U;
-  uint64_t bits = (bit0 ^ bit1) ^ (bit2 ^ bit3);
-  const uint64_t *pointToStart = points_radix_16 + (uint32_t)(bits * (uint64_t)(uint32_t)8U);
-  memcpy(resultBuffer, (uint64_t *)pointToStart, (uint32_t)8U * sizeof (uint64_t));
-  resultBuffer[8U] = (uint64_t)1U;
-  resultBuffer[9U] = (uint64_t)0U;
-  resultBuffer[10U] = (uint64_t)0U;
-  resultBuffer[11U] = (uint64_t)0U;
-  for (uint32_t i = (uint32_t)1U; i < (uint32_t)64U; i++)
+  uint32_t len20 = (uint32_t)6U;
+  uint64_t *x = q;
+  uint64_t *y = q + len20;
+  uint64_t *z = q + (uint32_t)2U * len20;
+  uint32_t len3 = (uint32_t)6U;
+  for (uint32_t i = (uint32_t)0U; i < len3; i++)
   {
-    uint64_t pointToAdd[8U] = { 0U };
-    getPointPrecomputedMixed_p256((void *)scalar, i, pointToAdd);
-    point_double_p384(resultBuffer, resultBuffer, buff);
-    point_double_p384(resultBuffer, resultBuffer, buff);
-    point_double_p384(resultBuffer, resultBuffer, buff);
-    point_double_p384(resultBuffer, resultBuffer, buff);
-    point_add_mixed_p384(resultBuffer, pointToAdd, resultBuffer, buff);
+    x[i] = (uint64_t)0U;
   }
-  memcpy(q, resultBuffer, (uint32_t)18U * sizeof (uint64_t));
+  uint32_t len30 = (uint32_t)6U;
+  for (uint32_t i = (uint32_t)0U; i < len30; i++)
+  {
+    y[i] = (uint64_t)0U;
+  }
+  uint32_t len31 = (uint32_t)6U;
+  for (uint32_t i = (uint32_t)0U; i < len31; i++)
+  {
+    z[i] = (uint64_t)0U;
+  }
+  resultBuffer[0U] = (uint64_t)0x3dd0756649c0b528U;
+  resultBuffer[1U] = (uint64_t)0x20e378e2a0d6ce38U;
+  resultBuffer[2U] = (uint64_t)0x879c3afc541b4d6eU;
+  resultBuffer[3U] = (uint64_t)0x6454868459a30effU;
+  resultBuffer[4U] = (uint64_t)0x812ff723614ede2bU;
+  resultBuffer[5U] = (uint64_t)0x4d3aadc2299e1513U;
+  resultBuffer[6U] = (uint64_t)0x23043dad4b03a4feU;
+  resultBuffer[7U] = (uint64_t)0xa1bfa8bf7bb4a9acU;
+  resultBuffer[8U] = (uint64_t)0x8bade7562e83b050U;
+  resultBuffer[9U] = (uint64_t)0xc6c3521968f4ffd9U;
+  resultBuffer[10U] = (uint64_t)0xdd8002263969a840U;
+  resultBuffer[11U] = (uint64_t)0x2b78abc25a15c5e9U;
+  resultBuffer[12U] = (uint64_t)0xffffffff00000001U;
+  resultBuffer[13U] = (uint64_t)0xffffffffU;
+  resultBuffer[14U] = (uint64_t)0x1U;
+  resultBuffer[15U] = (uint64_t)0U;
+  resultBuffer[16U] = (uint64_t)0U;
+  resultBuffer[17U] = (uint64_t)0U;
+  montgomery_ladderP384L(q, resultBuffer, scalar, buff);
   norm_p384(q, resultBuffer, buff);
   uint32_t len10 = (uint32_t)6U;
   uint32_t start = len10 * (uint32_t)2U;
@@ -14689,7 +14248,94 @@ uint64_t Hacl_P256_ecp384dh_i(uint8_t *result, uint8_t *scalar)
  Output: uint64, where 0 stands for the correct key generation. All the other values mean that an error has occurred. 
   
 */
-uint64_t Hacl_P256_ecp256dh_r(uint8_t *result, uint8_t *pubKey, uint8_t *scalar)
+uint64_t Hacl_P256_ecp256dh_r_ml(uint8_t *result, uint8_t *pubKey, uint8_t *scalar)
+{
+  uint32_t len = (uint32_t)4U;
+  KRML_CHECK_SIZE(sizeof (uint64_t), (uint32_t)3U * len);
+  uint64_t rF[(uint32_t)3U * len];
+  memset(rF, 0U, (uint32_t)3U * len * sizeof (uint64_t));
+  KRML_CHECK_SIZE(sizeof (uint64_t), (uint32_t)3U * len);
+  uint64_t pkF[(uint32_t)3U * len];
+  memset(pkF, 0U, (uint32_t)3U * len * sizeof (uint64_t));
+  toFormPoint_p256(pubKey, pkF);
+  uint32_t len1 = (uint32_t)4U;
+  KRML_CHECK_SIZE(sizeof (uint64_t), (uint32_t)20U * len1);
+  uint64_t tempBuffer[(uint32_t)20U * len1];
+  memset(tempBuffer, 0U, (uint32_t)20U * len1 * sizeof (uint64_t));
+  bool publicKeyCorrect = verifyQValidCurvePoint_p256(pkF);
+  bool flag;
+  if (publicKeyCorrect)
+  {
+    uint32_t len30 = (uint32_t)4U;
+    uint64_t *q = tempBuffer;
+    uint64_t *buff = tempBuffer + (uint32_t)3U * len30;
+    uint32_t len4 = (uint32_t)4U;
+    uint64_t *x = q;
+    uint64_t *y = q + len4;
+    uint64_t *z = q + (uint32_t)2U * len4;
+    uint32_t len5 = (uint32_t)4U;
+    for (uint32_t i = (uint32_t)0U; i < len5; i++)
+    {
+      x[i] = (uint64_t)0U;
+    }
+    uint32_t len50 = (uint32_t)4U;
+    for (uint32_t i = (uint32_t)0U; i < len50; i++)
+    {
+      y[i] = (uint64_t)0U;
+    }
+    uint32_t len51 = (uint32_t)4U;
+    for (uint32_t i = (uint32_t)0U; i < len51; i++)
+    {
+      z[i] = (uint64_t)0U;
+    }
+    uint32_t len40 = (uint32_t)4U;
+    uint64_t *p_x = pkF;
+    uint64_t *p_y = pkF + len40;
+    uint64_t *p_z = pkF + (uint32_t)2U * len40;
+    uint64_t *r_x = rF;
+    uint64_t *r_y = rF + len40;
+    uint64_t *r_z = rF + (uint32_t)2U * len40;
+    toDomain_p256(p_x, r_x);
+    toDomain_p256(p_y, r_y);
+    toDomain_p256(p_z, r_z);
+    montgomery_ladderP256L(q, rF, scalar, buff);
+    memcpy(rF, q, (uint32_t)12U * sizeof (uint64_t));
+    norm_p256(rF, rF, tempBuffer);
+    uint32_t len2 = (uint32_t)4U;
+    uint32_t start = len2 * (uint32_t)2U;
+    uint64_t *zCoordinate = rF + start;
+    uint64_t tmp = (uint64_t)18446744073709551615U;
+    uint32_t len3 = (uint32_t)4U;
+    for (uint32_t i = (uint32_t)0U; i < len3; i++)
+    {
+      uint64_t a_i = zCoordinate[i];
+      uint64_t r_i = FStar_UInt64_eq_mask(a_i, (uint64_t)0U);
+      uint64_t tmp0 = tmp;
+      tmp = r_i & tmp0;
+    }
+    uint64_t r = tmp;
+    uint64_t flag0 = r;
+    flag = flag0 == (uint64_t)0U;
+  }
+  else
+  {
+    flag = false;
+  }
+  fromFormPoint_p256(rF, result);
+  bool flag0 = flag;
+  return (uint64_t)flag0;
+}
+
+/*
+ This code is not side channel resistant on pub_key. 
+ Input: result: uint8[64], 
+ pub(lic)Key: uint8[64], 
+ scalar: uint8[32].
+  
+ Output: uint64, where 0 stands for the correct key generation. All the other values mean that an error has occurred. 
+  
+*/
+uint64_t Hacl_P256_ecp256dh_r_radix(uint8_t *result, uint8_t *pubKey, uint8_t *scalar)
 {
   uint32_t len = (uint32_t)4U;
   KRML_CHECK_SIZE(sizeof (uint64_t), (uint32_t)3U * len);
@@ -14875,127 +14521,43 @@ uint64_t Hacl_P256_ecp384dh_r(uint8_t *result, uint8_t *pubKey, uint8_t *scalar)
   uint64_t tempBuffer[(uint32_t)20U * len1];
   memset(tempBuffer, 0U, (uint32_t)20U * len1 * sizeof (uint64_t));
   bool publicKeyCorrect = verifyQValidCurvePoint_p384(pkF);
-  uint64_t bufferPrecomputed[192U];
   bool flag;
   if (publicKeyCorrect)
   {
+    uint32_t len30 = (uint32_t)6U;
+    uint64_t *q = tempBuffer;
+    uint64_t *buff = tempBuffer + (uint32_t)3U * len30;
     uint32_t len4 = (uint32_t)6U;
+    uint64_t *x = q;
+    uint64_t *y = q + len4;
+    uint64_t *z = q + (uint32_t)2U * len4;
+    uint32_t len5 = (uint32_t)6U;
+    for (uint32_t i = (uint32_t)0U; i < len5; i++)
+    {
+      x[i] = (uint64_t)0U;
+    }
+    uint32_t len50 = (uint32_t)6U;
+    for (uint32_t i = (uint32_t)0U; i < len50; i++)
+    {
+      y[i] = (uint64_t)0U;
+    }
+    uint32_t len51 = (uint32_t)6U;
+    for (uint32_t i = (uint32_t)0U; i < len51; i++)
+    {
+      z[i] = (uint64_t)0U;
+    }
+    uint32_t len40 = (uint32_t)6U;
     uint64_t *p_x = pkF;
-    uint64_t *p_y = pkF + len4;
-    uint64_t *p_z = pkF + (uint32_t)2U * len4;
+    uint64_t *p_y = pkF + len40;
+    uint64_t *p_z = pkF + (uint32_t)2U * len40;
     uint64_t *r_x = rF;
-    uint64_t *r_y = rF + len4;
-    uint64_t *r_z = rF + (uint32_t)2U * len4;
+    uint64_t *r_y = rF + len40;
+    uint64_t *r_z = rF + (uint32_t)2U * len40;
     toDomain_p384(p_x, r_x);
     toDomain_p384(p_y, r_y);
     toDomain_p384(p_z, r_z);
-    uint64_t init = (uint64_t)0U;
-    for (uint32_t i = (uint32_t)0U; i < (uint32_t)192U; i++)
-    {
-      bufferPrecomputed[i] = init;
-    }
-    generatePrecomputedTable(Spec_ECC_Curves_P384, bufferPrecomputed, rF, tempBuffer);
-    uint32_t
-    bit = (uint32_t)6U * (uint32_t)8U * (uint32_t)8U - (uint32_t)1U - (uint32_t)(uint64_t)0U;
-    uint64_t
-    bit00 =
-      (uint64_t)(scalar[(uint32_t)6U
-      * (uint32_t)8U
-      - (uint32_t)1U
-      - bit / (uint32_t)8U]
-      >> bit % (uint32_t)8U
-      & (uint8_t)1U)
-      << (uint32_t)3U;
-    uint64_t
-    bit10 =
-      (uint64_t)(scalar[(uint32_t)6U
-      * (uint32_t)8U
-      - (uint32_t)1U
-      - (bit - (uint32_t)1U) / (uint32_t)8U]
-      >> (bit - (uint32_t)1U) % (uint32_t)8U
-      & (uint8_t)1U)
-      << (uint32_t)2U;
-    uint64_t
-    bit20 =
-      (uint64_t)(scalar[(uint32_t)6U
-      * (uint32_t)8U
-      - (uint32_t)1U
-      - (bit - (uint32_t)2U) / (uint32_t)8U]
-      >> (bit - (uint32_t)2U) % (uint32_t)8U
-      & (uint8_t)1U)
-      << (uint32_t)1U;
-    uint64_t
-    bit30 =
-      (uint64_t)(scalar[(uint32_t)6U
-      * (uint32_t)8U
-      - (uint32_t)1U
-      - (bit - (uint32_t)3U) / (uint32_t)8U]
-      >> (bit - (uint32_t)3U) % (uint32_t)8U
-      & (uint8_t)1U)
-      << (uint32_t)0U;
-    uint64_t bits = (bit00 ^ bit10) ^ (bit20 ^ bit30);
-    uint64_t *pointToStart = bufferPrecomputed + (uint32_t)(bits * (uint64_t)(uint32_t)12U);
-    memcpy(rF, pointToStart, (uint32_t)12U * sizeof (uint64_t));
-    for (uint32_t i0 = (uint32_t)1U; i0 < (uint32_t)64U; i0++)
-    {
-      uint32_t
-      bit4 = (uint32_t)6U * (uint32_t)8U * (uint32_t)8U - (uint32_t)1U - (i0 << (uint32_t)2U);
-      uint64_t
-      bit0 =
-        (uint64_t)(scalar[(uint32_t)6U
-        * (uint32_t)8U
-        - (uint32_t)1U
-        - bit4 / (uint32_t)8U]
-        >> bit4 % (uint32_t)8U
-        & (uint8_t)1U)
-        << (uint32_t)3U;
-      uint64_t
-      bit1 =
-        (uint64_t)(scalar[(uint32_t)6U
-        * (uint32_t)8U
-        - (uint32_t)1U
-        - (bit4 - (uint32_t)1U) / (uint32_t)8U]
-        >> (bit4 - (uint32_t)1U) % (uint32_t)8U
-        & (uint8_t)1U)
-        << (uint32_t)2U;
-      uint64_t
-      bit2 =
-        (uint64_t)(scalar[(uint32_t)6U
-        * (uint32_t)8U
-        - (uint32_t)1U
-        - (bit4 - (uint32_t)2U) / (uint32_t)8U]
-        >> (bit4 - (uint32_t)2U) % (uint32_t)8U
-        & (uint8_t)1U)
-        << (uint32_t)1U;
-      uint64_t
-      bit3 =
-        (uint64_t)(scalar[(uint32_t)6U
-        * (uint32_t)8U
-        - (uint32_t)1U
-        - (bit4 - (uint32_t)3U) / (uint32_t)8U]
-        >> (bit4 - (uint32_t)3U) % (uint32_t)8U
-        & (uint8_t)1U)
-        << (uint32_t)0U;
-      uint64_t bits1 = (bit0 ^ bit1) ^ (bit2 ^ bit3);
-      uint64_t pointToAdd[12U] = { 0U };
-      for (uint32_t i = (uint32_t)0U; i < (uint32_t)16U; i++)
-      {
-        uint64_t mask = FStar_UInt64_eq_mask(bits1, (uint64_t)i);
-        uint64_t *lut_cmb_x = bufferPrecomputed + i * (uint32_t)(krml_checked_int_t)12;
-        uint64_t
-        *lut_cmb_y = bufferPrecomputed + i * (uint32_t)(krml_checked_int_t)12 + (uint32_t)4U;
-        uint64_t
-        *lut_cmb_z = bufferPrecomputed + i * (uint32_t)(krml_checked_int_t)12 + (uint32_t)8U;
-        copy_conditional_p384_l(pointToAdd, lut_cmb_x, mask);
-        copy_conditional_p384_l(pointToAdd + (uint32_t)4U, lut_cmb_y, mask);
-        copy_conditional_p384_l(pointToAdd + (uint32_t)8U, lut_cmb_z, mask);
-      }
-      point_double_p256(rF, rF, tempBuffer);
-      point_double_p256(rF, rF, tempBuffer);
-      point_double_p256(rF, rF, tempBuffer);
-      point_double_p256(rF, rF, tempBuffer);
-      point_add_p256(pointToAdd, rF, rF, tempBuffer);
-    }
+    montgomery_ladderP384L(q, rF, scalar, buff);
+    memcpy(rF, q, (uint32_t)18U * sizeof (uint64_t));
     norm_p384(rF, rF, tempBuffer);
     uint32_t len2 = (uint32_t)6U;
     uint32_t start = len2 * (uint32_t)2U;
