code/ecdsa/dist/test.c
@@ -1,0 +1,439 @@
+#include <inttypes.h>
+#include <stdio.h>
+#include <stdlib.h>
+#include <string.h>
+#include <sys/types.h>
+#include <sys/stat.h>
+#include <fcntl.h>
+#include <unistd.h>
+#include <time.h>
+#include <stdbool.h>
+#include "test_helpers.h"
+
+#include "Hacl_P256.h"
+
+#include <stdint.h>
+#include <string.h>
+#include <stdint.h>
+
+
+
+#define SIZE   32
+#define ROUNDS 10000
+
+static inline bool compare(size_t len, uint8_t* comp, uint8_t* exp) {
+  bool ok = true;
+  for (size_t i = 0; i < len; i++)
+    ok = ok & (exp[i] == comp[i]);
+  return ok;
+}
+
+
+#include <assert.h>
+
+
+void hex2bytes(unsigned char *out, const char *in) {
+    int i;
+    int len = strlen(in);
+
+    assert(out != NULL);
+    assert(in != NULL);
+    assert(len == 64);
+
+    for (i = len - 2; i >= 0; i -= 2, out++)
+        assert(sscanf(in + i, "%02hhx", out) == 1);
+}
+
+
+#define MP_BE2LE(a)            \
+    do {                       \
+        unsigned char z_bswap; \
+        z_bswap = a[0];        \
+        a[0] = a[31];          \
+        a[31] = z_bswap;       \
+        z_bswap = a[1];        \
+        a[1] = a[30];          \
+        a[30] = z_bswap;       \
+        z_bswap = a[2];        \
+        a[2] = a[29];          \
+        a[29] = z_bswap;       \
+        z_bswap = a[3];        \
+        a[3] = a[28];          \
+        a[28] = z_bswap;       \
+        z_bswap = a[4];        \
+        a[4] = a[27];          \
+        a[27] = z_bswap;       \
+        z_bswap = a[5];        \
+        a[5] = a[26];          \
+        a[26] = z_bswap;       \
+        z_bswap = a[6];        \
+        a[6] = a[25];          \
+        a[25] = z_bswap;       \
+        z_bswap = a[7];        \
+        a[7] = a[24];          \
+        a[24] = z_bswap;       \
+        z_bswap = a[8];        \
+        a[8] = a[23];          \
+        a[23] = z_bswap;       \
+        z_bswap = a[9];        \
+        a[9] = a[22];          \
+        a[22] = z_bswap;       \
+        z_bswap = a[10];       \
+        a[10] = a[21];         \
+        a[21] = z_bswap;       \
+        z_bswap = a[11];       \
+        a[11] = a[20];         \
+        a[20] = z_bswap;       \
+        z_bswap = a[12];       \
+        a[12] = a[19];         \
+        a[19] = z_bswap;       \
+        z_bswap = a[13];       \
+        a[13] = a[18];         \
+        a[18] = z_bswap;       \
+        z_bswap = a[14];       \
+        a[14] = a[17];         \
+        a[17] = z_bswap;       \
+        z_bswap = a[15];       \
+        a[15] = a[16];         \
+        a[16] = z_bswap;       \
+    } while (0)
+
+
+
+bool test_ecdh()
+{
+
+    static uint8_t publicKeyX1[32] = {
+    0x70, 0x0c, 0x48, 0xf7, 0x7f, 0x56, 0x58, 0x4c, 0x5c, 0xc6, 0x32, 0xca, 0x65, 0x64, 0x0d, 0xb9, 0x1b, 0x6b, 0xac, 0xce, 0x3a, 0x4d, 0xf6, 0xb4, 0x2c, 0xe7, 0xcc, 0x83, 0x88, 0x33, 0xd2, 0x87 
+    };
+
+    static uint8_t publicKeyY1[32] = {
+    0xdb, 0x71, 0xe5, 0x09, 0xe3, 0xfd, 0x9b, 0x06, 0x0d, 0xdb, 0x20, 0xba, 0x5c, 0x51, 0xdc, 0xc5, 0x94, 0x8d, 0x46, 0xfb, 0xf6, 0x40, 0xdf, 0xe0, 0x44, 0x17, 0x82, 0xca, 0xb8, 0x5f, 0xa4, 0xac 
+    };
+    
+    static uint8_t privateKey[32] = {
+    0x7d, 0x7d, 0xc5, 0xf7, 0x1e, 0xb2, 0x9d, 0xda, 0xf8, 0x0d, 0x62, 0x14, 0x63, 0x2e, 0xea, 0xe0, 0x3d, 0x90, 0x58, 0xaf, 0x1f, 0xb6, 0xd2, 0x2e, 0xd8, 0x0b, 0xad, 0xb6, 0x2b, 0xc1, 0xa5, 0x34 
+    };
+
+    static uint8_t expectedPublicKeyX[32] = {
+    0xea, 0xd2, 0x18, 0x59, 0x01, 0x19, 0xe8, 0x87, 0x6b, 0x29, 0x14, 0x6f, 0xf8, 0x9c, 0xa6, 0x17, 0x70, 0xc4, 0xed, 0xbb, 0xf9, 0x7d, 0x38, 0xce, 0x38, 0x5e, 0xd2, 0x81, 0xd8, 0xa6, 0xb2, 0x30 
+    };
+    
+    static uint8_t expectedPublicKeyY[32] = {
+    0x28, 0xaf, 0x61, 0x28, 0x1f, 0xd3, 0x5e, 0x2f, 0xa7, 0x00, 0x25, 0x23, 0xac, 0xc8, 0x5a, 0x42, 0x9c, 0xb0, 0x6e, 0xe6, 0x64, 0x83, 0x25, 0x38, 0x9f, 0x59, 0xed, 0xfc, 0xe1, 0x40, 0x51, 0x41 
+    };
+
+    static uint8_t expectedResult[32] = {
+    0x46, 0xfc, 0x62, 0x10, 0x64, 0x20, 0xff, 0x01, 0x2e, 0x54, 0xa4, 0x34, 0xfb, 0xdd, 0x2d, 0x25, 0xcc, 0xc5, 0x85, 0x20, 0x60, 0x56, 0x1e, 0x68, 0x04, 0x0d, 0xd7, 0x77, 0x89, 0x97, 0xbd, 0x7b 
+    };
+
+    bool ok = true;
+
+    printf("%s\n", "---------------------------------------------------------------" );
+
+    printf("%s\n", "ECDH Initiator");
+
+
+
+    uint8_t* result = (uint8_t*) malloc (sizeof (uint8_t) * 64);
+    uint8_t* pk = (uint8_t*) malloc (sizeof (uint8_t) * 64);
+    
+    
+    bool successDHI = Hacl_P256_ecp256dh_i_ml(result, privateKey);
+    printf("\n");
+    ok = ok && successDHI;
+    compare_and_print(32, result, expectedPublicKeyX);
+    compare_and_print(32, result + 32, expectedPublicKeyY);
+    
+
+    printf("%s\n", "---------------------------------------------------------------" );
+
+    printf("%s\n", "ECDH Initiator - Radix");
+
+
+
+    uint8_t* result_i_radix = (uint8_t*) malloc (sizeof (uint8_t) * 64);
+    
+    successDHI = Hacl_P256_ecp256dh_i_radix(result_i_radix, privateKey);
+    printf("\n");
+    ok = ok && successDHI;
+    compare_and_print(32, result_i_radix, expectedPublicKeyX);
+    compare_and_print(32, result_i_radix + 32, expectedPublicKeyY);
+
+
+    printf("\n");
+
+    printf("%s\n", "---------------------------------------------------------------" );
+
+    printf("%s\n", "ECDH Responder");
+
+
+    result = (uint8_t*) malloc (sizeof (uint8_t) * 64);
+    memcpy(pk, publicKeyX1,  32);
+    memcpy(pk+32, publicKeyY1,  32);
+       
+    bool successDHR = Hacl_P256_ecp256dh_r_ml(result, pk, privateKey);
+    ok = ok && compare_and_print(32, result, expectedResult);
+    ok = ok && successDHR;
+
+
+    printf("%s\n", "---------------------------------------------------------------" );
+
+    printf("%s\n", "ECDH Responder Radix");
+
+
+    result = (uint8_t*) malloc (sizeof (uint8_t) * 64);
+    memcpy(pk, publicKeyX1,  32);
+    memcpy(pk+32, publicKeyY1,  32);
+       
+    successDHR = Hacl_P256_ecp256dh_r_radix(result, pk, privateKey);
+    ok = ok && compare_and_print(32, result, expectedResult);
+    ok = ok && successDHR;
+
+
+
+    return ok;
+}
+
+
+
+
+void master_branch_test()
+{
+	cycles a,b;
+	clock_t t1,t2;
+	uint8_t* result = (uint8_t*) malloc (sizeof (uint8_t) * 32);
+
+	uint64_t len = SIZE;
+
+	uint8_t scalar[SIZE];
+	memset(scalar,'P',SIZE);
+	
+  	for (int j = 0; j < ROUNDS; j++)
+		Hacl_P256_ecp256dh_i_ml(result, scalar);
+
+	t1 = clock();
+  	a = cpucycles_begin();
+
+  	for (int j = 0; j < ROUNDS; j++)
+		Hacl_P256_ecp256dh_i_ml(result, scalar);
+	
+	b = cpucycles_end();
+	
+	t2 = clock();
+	clock_t tdiff1 = t2 - t1;
+	cycles cdiff1 = b - a;
+
+	double time = (((double)tdiff1) / CLOCKS_PER_SEC);
+	double nsigs = ((double)ROUNDS) / time;
+	printf("HACL P-256 [SecretToPublic] PERF Ladder \n");
+	printf("ECDH %8.2f mul/s\n",nsigs);
+
+  	printf("cycles per function call:  %" PRIu64 " \n \n",(uint64_t)cdiff1/ROUNDS);
+
+
+    static uint8_t publicKeyX1[32] = {
+    0x70, 0x0c, 0x48, 0xf7, 0x7f, 0x56, 0x58, 0x4c, 0x5c, 0xc6, 0x32, 0xca, 0x65, 0x64, 0x0d, 0xb9, 0x1b, 0x6b, 0xac, 0xce, 0x3a, 0x4d, 0xf6, 0xb4, 0x2c, 0xe7, 0xcc, 0x83, 0x88, 0x33, 0xd2, 0x87 
+    };
+
+    static uint8_t publicKeyY1[32] = {
+    0xdb, 0x71, 0xe5, 0x09, 0xe3, 0xfd, 0x9b, 0x06, 0x0d, 0xdb, 0x20, 0xba, 0x5c, 0x51, 0xdc, 0xc5, 0x94, 0x8d, 0x46, 0xfb, 0xf6, 0x40, 0xdf, 0xe0, 0x44, 0x17, 0x82, 0xca, 0xb8, 0x5f, 0xa4, 0xac 
+    };
+    
+    static uint8_t privateKey[32] = {
+    0x7d, 0x7d, 0xc5, 0xf7, 0x1e, 0xb2, 0x9d, 0xda, 0xf8, 0x0d, 0x62, 0x14, 0x63, 0x2e, 0xea, 0xe0, 0x3d, 0x90, 0x58, 0xaf, 0x1f, 0xb6, 0xd2, 0x2e, 0xd8, 0x0b, 0xad, 0xb6, 0x2b, 0xc1, 0xa5, 0x34 
+    };
+
+    static uint8_t expectedPublicKeyX[32] = {
+    0xea, 0xd2, 0x18, 0x59, 0x01, 0x19, 0xe8, 0x87, 0x6b, 0x29, 0x14, 0x6f, 0xf8, 0x9c, 0xa6, 0x17, 0x70, 0xc4, 0xed, 0xbb, 0xf9, 0x7d, 0x38, 0xce, 0x38, 0x5e, 0xd2, 0x81, 0xd8, 0xa6, 0xb2, 0x30 
+    };
+    
+    static uint8_t expectedPublicKeyY[32] = {
+    0x28, 0xaf, 0x61, 0x28, 0x1f, 0xd3, 0x5e, 0x2f, 0xa7, 0x00, 0x25, 0x23, 0xac, 0xc8, 0x5a, 0x42, 0x9c, 0xb0, 0x6e, 0xe6, 0x64, 0x83, 0x25, 0x38, 0x9f, 0x59, 0xed, 0xfc, 0xe1, 0x40, 0x51, 0x41 
+    };
+
+    static uint8_t expectedResult[32] = {
+    0x46, 0xfc, 0x62, 0x10, 0x64, 0x20, 0xff, 0x01, 0x2e, 0x54, 0xa4, 0x34, 0xfb, 0xdd, 0x2d, 0x25, 0xcc, 0xc5, 0x85, 0x20, 0x60, 0x56, 0x1e, 0x68, 0x04, 0x0d, 0xd7, 0x77, 0x89, 0x97, 0xbd, 0x7b 
+    };
+
+
+	uint8_t* pk = (uint8_t*) malloc (sizeof (uint8_t) * 64);
+	
+	memcpy(pk, publicKeyX1,  32);
+	memcpy(pk+32, publicKeyY1,  32);
+
+	for (int j = 0; j < ROUNDS; j++)
+		Hacl_P256_ecp256dh_r_ml(result, pk, privateKey);
+
+
+	t1 = clock();
+  	a = cpucycles_begin();
+
+  	for (int j = 0; j < ROUNDS; j++)
+		Hacl_P256_ecp256dh_r_ml(result, pk, privateKey);
+	
+	b = cpucycles_end();
+	
+	t2 = clock();
+	clock_t tdiff6 = t2 - t1;
+
+	double timeLadderR = (((double)tdiff6) / CLOCKS_PER_SEC);
+	double nsigsLadderR = ((double)ROUNDS) / timeLadderR;
+	printf("HACL P-256 ECDH [Scalar Multiplication] PERF Ladder \n");
+	printf("ECDH %8.2f mul/s\n",nsigsLadderR);
+
+	cycles cdiff6 = b - a;
+  	printf("cycles per function call:  %" PRIu64 " \n \n",(uint64_t)cdiff6/ROUNDS);
+
+}
+
+bool test_ecdsa()
+{
+    uint8_t* pk = (uint8_t*) malloc (sizeof (uint8_t) * 64);
+    bool ok = true;
+
+    static uint8_t pkx_0  [32] = { 
+    0x29, 0x27, 0xb1, 0x05, 0x12, 0xba, 0xe3, 0xed, 0xdc, 0xfe, 0x46, 0x78, 0x28, 0x12, 0x8b, 0xad, 0x29, 0x03, 0x26, 0x99, 0x19, 0xf7, 0x08, 0x60, 0x69, 0xc8, 0xc4, 0xdf, 0x6c, 0x73, 0x28, 0x38}; 
+
+    static uint8_t pky_0  [32] = {
+    0xc7, 0x78, 0x79, 0x64, 0xea, 0xac, 0x00, 0xe5, 0x92, 0x1f, 0xb1, 0x49, 0x8a, 0x60, 0xf4, 0x60, 0x67, 0x66, 0xb3, 0xd9, 0x68, 0x50, 0x01, 0x55, 0x8d, 0x1a, 0x97, 0x4e, 0x73, 0x41, 0x51, 0x3e};
+
+    #define mLen0 6 
+
+    static uint8_t msg_0  [6] = {
+    0x31, 0x32, 0x33, 0x34, 0x30, 0x30
+    }; 
+
+    static uint8_t r_0  [32] = {
+    0x2b, 0xa3, 0xa8, 0xbe, 0x6b, 0x94, 0xd5, 0xec, 0x80, 0xa6, 0xd9, 0xd1, 0x19, 0x0a, 0x43, 0x6e, 0xff, 0xe5, 0x0d, 0x85, 0xa1, 0xee, 0xe8, 0x59, 0xb8, 0xcc, 0x6a, 0xf9, 0xbd, 0x5c, 0x2e, 0x18
+    }; 
+
+    static uint8_t s_0  [32] = {
+    0x4c, 0xd6, 0x0b, 0x85, 0x5d, 0x44, 0x2f, 0x5b, 0x3c, 0x7b, 0x11, 0xeb, 0x6c, 0x4e, 0x0a, 0xe7, 0x52, 0x5f, 0xe7, 0x10, 0xfa, 0xb9, 0xaa, 0x7c, 0x77, 0xa6, 0x7f, 0x79, 0xe6, 0xfa, 0xdd, 0x76
+    }; 
+
+    #define result___0 0
+
+    memcpy(pk, pkx_0, 32);
+    memcpy(pk + 32, pky_0, 32);
+
+
+    bool verificationSuccessful = Hacl_P256_ecdsa_verif_p256_sha2(mLen0, msg_0, pk, r_0, s_0);    
+    if (verificationSuccessful)  
+     {
+        printf("%s\n", "Verification success");
+     ok = true;
+     }
+        else
+    { 
+         printf("%s\n", "Verification Failed");
+        ok = false;
+
+    }
+
+
+
+    uint8_t
+    prKey[32U] =
+      {
+        (uint8_t)81U, (uint8_t)155U, (uint8_t)66U, (uint8_t)61U, (uint8_t)113U, (uint8_t)95U,
+        (uint8_t)139U, (uint8_t)88U, (uint8_t)31U, (uint8_t)79U, (uint8_t)168U, (uint8_t)238U,
+        (uint8_t)89U, (uint8_t)244U, (uint8_t)119U, (uint8_t)26U, (uint8_t)91U, (uint8_t)68U,
+        (uint8_t)200U, (uint8_t)19U, (uint8_t)11U, (uint8_t)78U, (uint8_t)62U, (uint8_t)172U,
+        (uint8_t)202U, (uint8_t)84U, (uint8_t)165U, (uint8_t)109U, (uint8_t)218U, (uint8_t)114U,
+        (uint8_t)180U, (uint8_t)100U
+      };
+
+    uint8_t
+    digest[32U] =
+      {
+        (uint8_t)28U, (uint8_t)203U, (uint8_t)233U, (uint8_t)28U, (uint8_t)7U, (uint8_t)95U,
+        (uint8_t)199U, (uint8_t)244U, (uint8_t)240U, (uint8_t)51U, (uint8_t)191U, (uint8_t)162U,
+        (uint8_t)72U, (uint8_t)219U, (uint8_t)143U, (uint8_t)204U, (uint8_t)211U, (uint8_t)86U,
+        (uint8_t)93U, (uint8_t)233U, (uint8_t)75U, (uint8_t)191U, (uint8_t)177U, (uint8_t)47U,
+        (uint8_t)60U, (uint8_t)89U, (uint8_t)255U, (uint8_t)70U, (uint8_t)194U, (uint8_t)113U,
+        (uint8_t)191U, (uint8_t)131U
+      };
+
+    uint8_t
+    nonce[32U] =
+      {
+        (uint8_t)148U, (uint8_t)161U, (uint8_t)187U, (uint8_t)177U, (uint8_t)75U, (uint8_t)144U,
+        (uint8_t)106U, (uint8_t)97U, (uint8_t)162U, (uint8_t)128U, (uint8_t)242U, (uint8_t)69U,
+        (uint8_t)249U, (uint8_t)233U, (uint8_t)60U, (uint8_t)127U, (uint8_t)59U, (uint8_t)74U,
+        (uint8_t)98U, (uint8_t)71U, (uint8_t)130U, (uint8_t)79U, (uint8_t)93U, (uint8_t)51U,
+        (uint8_t)185U, (uint8_t)103U, (uint8_t)7U, (uint8_t)135U, (uint8_t)100U, (uint8_t)42U,
+        (uint8_t)104U, (uint8_t)222U
+      };
+
+    uint8_t
+    siggen_vectors_low5[32U] =
+      {
+        (uint8_t)243U, (uint8_t)172U, (uint8_t)128U, (uint8_t)97U, (uint8_t)181U, (uint8_t)20U,
+        (uint8_t)121U, (uint8_t)91U, (uint8_t)136U, (uint8_t)67U, (uint8_t)227U, (uint8_t)214U,
+        (uint8_t)98U, (uint8_t)149U, (uint8_t)39U, (uint8_t)237U, (uint8_t)42U, (uint8_t)253U,
+        (uint8_t)107U, (uint8_t)31U, (uint8_t)106U, (uint8_t)85U, (uint8_t)90U, (uint8_t)122U,
+        (uint8_t)202U, (uint8_t)187U, (uint8_t)94U, (uint8_t)111U, (uint8_t)121U, (uint8_t)200U,
+        (uint8_t)194U, (uint8_t)172U
+      };
+
+    uint8_t
+    siggen_vectors_low6[32U] =
+      {
+        0xcf, 0xa7, 0x40, 0xfe, 0xc7, 0x67, 0x96, 0xd2, 
+        0xe3, 0x92, 0x16, 0xbe, 0x7e, 0xbf, 0x58, 0x0e, 
+        0xa3, 0xc0, 0xef, 0x4b, 0xb0, 0x0a, 0xb2, 0xe7, 
+        0xe4, 0x20, 0x84, 0x34, 0xf4, 0x5f, 0x8c, 0x9c
+      };
+
+
+    static uint8_t px0_0[32] = {
+    0x70, 0x0c, 0x48, 0xf7, 0x7f, 0x56, 0x58, 0x4c, 0x5c, 0xc6, 0x32, 0xca, 0x65, 0x64, 0x0d, 0xb9, 0x1b, 0x6b, 0xac, 0xce, 0x3a, 0x4d, 0xf6, 0xb4, 0x2c, 0xe7, 0xcc, 0x83, 0x88, 0x33, 0xd2, 0x87 
+
+    };
+    static uint8_t py0_0[32] = {
+    0xdb, 0x71, 0xe5, 0x09, 0xe3, 0xfd, 0x9b, 0x06, 0x0d, 0xdb, 0x20, 0xba, 0x5c, 0x51, 0xdc, 0xc5, 0x94, 0x8d, 0x46, 0xfb, 0xf6, 0x40, 0xdf, 0xe0, 0x44, 0x17, 0x82, 0xca, 0xb8, 0x5f, 0xa4, 0xac 
+    };
+
+    static uint8_t scalar0[32] = {
+    0x7d, 0x7d, 0xc5, 0xf7, 0x1e, 0xb2, 0x9d, 0xda, 0xf8, 0x0d, 0x62, 0x14, 0x63, 0x2e, 0xea, 0xe0, 0x3d, 0x90, 0x58, 0xaf, 0x1f, 0xb6, 0xd2, 0x2e, 0xd8, 0x0b, 0xad, 0xb6, 0x2b, 0xc1, 0xa5, 0x34 
+
+    };
+
+
+
+
+
+    uint8_t* result = (uint8_t*) malloc (sizeof (uint8_t) * 64);
+    bool flag = Hacl_P256_ecdsa_sign_p256_without_hash(result, 32, digest, prKey, nonce);
+    bool s0 = compare_and_print(32, result, siggen_vectors_low5);
+    bool s1 = compare_and_print(32, result + 32, siggen_vectors_low6);
+
+    return ok && s0 && s1 && flag;
+}
+
+
+
+
+
+
+int main()
+{
+
+    if (test_ecdh () == false)
+        printf("%s\n", "WRONG"); 
+    if (test_ecdsa () == false)
+        printf("%s\n", "WRONG"); 
+
+
+	// master_branch_test();
+}
+
+// #include <inttypes.h>
+// void printU(uint64_t* t, int len)
+// {
+//   for (int i = 0; i< len; i++) {
+//     printf("%016llX ", t[i]);  
+//   }
+//   printf("\n");
+// }
