code/ecdsa/Hacl.P256.fst
@@ -31,33 +31,33 @@ open Hacl.Impl.EC.Core
 
 
 let ecdsa_sign_p256_sha2 result mLen m privKey k = 
-  ecdsa_signature #P256 (Hash SHA2_256) result mLen m privKey k
+  ecdsa_signature #P256 #ML (Hash SHA2_256) result mLen m privKey k
 
   let ecdsa_sign_p256_sha384 result mLen m privKey k = 
-  ecdsa_signature #P256 (Hash SHA2_384) result mLen m privKey k
+  ecdsa_signature #P256 #ML (Hash SHA2_384) result mLen m privKey k
 
 let ecdsa_sign_p256_sha512 result mLen m privKey k = 
-  ecdsa_signature #P256 (Hash SHA2_512) result mLen m privKey k
+  ecdsa_signature #P256 #ML (Hash SHA2_512) result mLen m privKey k
 
 let ecdsa_sign_p256_without_hash result mLen m privKey k = 
-  ecdsa_signature #P256 NoHash result mLen m privKey k
+  ecdsa_signature #P256 #ML NoHash result mLen m privKey k
 
 
 let ecdsa_verif_p256_sha2 mLen m pubKey r s = 
-  ecdsa_verification #P256 (Hash SHA2_256) pubKey r s mLen m
+  ecdsa_verification #P256 #ML (Hash SHA2_256) pubKey r s mLen m
 
 let ecdsa_verif_p256_sha384 mLen m pubKey r s = 
-  ecdsa_verification #P256 (Hash SHA2_384) pubKey r s mLen m
+  ecdsa_verification #P256 #ML (Hash SHA2_384) pubKey r s mLen m
 
 let ecdsa_verif_p256_sha512 mLen m pubKey r s = 
-  ecdsa_verification #P256 (Hash SHA2_512) pubKey r s mLen m
+  ecdsa_verification #P256 #ML (Hash SHA2_512) pubKey r s mLen m
 
 let ecdsa_verif_without_hash mLen m pubKey r s  =
-   ecdsa_verification #P256 NoHash pubKey r s mLen m
+   ecdsa_verification #P256 #ML NoHash pubKey r s mLen m
 
 
 let verify_q pubKey = 
-    Hacl.Impl.P256.Signature.Common.verifyQ #P256 pubKey
+    Hacl.Impl.P256.Signature.Common.verifyQ #P256 #ML pubKey
 
 (*)
 let decompression_not_compressed_form b result = 
@@ -84,7 +84,10 @@ let ecp256dh_i_radix result scalar = Hacl.Impl.EC.DH.ecp256dh_i P256 Radix resul
 
 let ecp384dh_i result scalar = Hacl.Impl.EC.DH.ecp256dh_i P384 ML result scalar
 
-let ecp256dh_r result pubKey scalar = Hacl.Impl.EC.DH.ecp256dh_r #P256 result pubKey scalar
+let ecp256dh_r_ml result pubKey scalar = Hacl.Impl.EC.DH.ecp256dh_r #P256 #ML result pubKey scalar
 
-let ecp384dh_r result pubKey scalar = Hacl.Impl.EC.DH.ecp256dh_r #P384 result pubKey scalar
+let ecp256dh_r_radix result pubKey scalar = Hacl.Impl.EC.DH.ecp256dh_r #P256 #Radix result pubKey scalar
+
+
+let ecp384dh_r result pubKey scalar = Hacl.Impl.EC.DH.ecp256dh_r #P384 #ML result pubKey scalar
 
