code/ecdsa/Hacl.P256.fsti
@@ -401,7 +401,7 @@ val ecp384dh_i:
 [@ (Comment " This code is not side channel resistant on pub_key. \n Input: result: uint8[64], \n pub(lic)Key: uint8[64], \n scalar: uint8[32].
   \n Output: uint64, where 0 stands for the correct key generation. All the other values mean that an error has occurred. 
   ")] 
-val ecp256dh_r:
+val ecp256dh_r_ml:
     result:lbuffer uint8 (size 64)
   -> pubKey:lbuffer uint8 (size 64)
   -> scalar:lbuffer uint8 (size 32)
@@ -418,6 +418,29 @@ val ecp256dh_r:
       modifies (loc result) h0 h1 /\
       as_seq h1 (gsub result (size 0) (size 32)) == pointX /\
       as_seq h1 (gsub result (size 32) (size 32)) == pointY)
+
+
+[@ (Comment " This code is not side channel resistant on pub_key. \n Input: result: uint8[64], \n pub(lic)Key: uint8[64], \n scalar: uint8[32].
+  \n Output: uint64, where 0 stands for the correct key generation. All the other values mean that an error has occurred. 
+  ")] 
+val ecp256dh_r_radix:
+    result:lbuffer uint8 (size 64)
+  -> pubKey:lbuffer uint8 (size 64)
+  -> scalar:lbuffer uint8 (size 32)
+  -> Stack uint64
+    (requires fun h ->
+      live h result /\ live h pubKey /\ live h scalar /\
+      disjoint result pubKey /\ disjoint result scalar)
+    (ensures fun h0 r h1 ->
+      let pubKeyX = gsub pubKey (size 0) (size 32) in
+      let pubKeyY = gsub pubKey (size 32) (size 32) in
+      let pointX, pointY, flag =
+        ecp256_dh_r #P256 (as_seq h0 pubKeyX) (as_seq h0 pubKeyY) (as_seq h0 scalar) in
+      r == flag /\
+      modifies (loc result) h0 h1 /\
+      as_seq h1 (gsub result (size 0) (size 32)) == pointX /\
+      as_seq h1 (gsub result (size 32) (size 32)) == pointY)
+
 
 
 [@ (Comment " This code is not side channel resistant on pub_key. \n Input: result: uint8[64], \n pub(lic)Key: uint8[64], \n scalar: uint8[32].
